vType_index_free -> vType: rename, as it is now stable

theories/νType/νType.v
@@ -1,97 +1,45 @@
-(** An "indexed" construction of ν-parametric sets
-    For ν=1, this builds augmented semi-simplicial sets
-    For ν=2, this builds semi-cubical sets *)
-
-Import Logic.EqNotations.
+Require Import List.
+Import Logic.EqNotations ListNotations.
 Require Import Logic.FunctionalExtensionality.
 
 Set Warnings "-notation-overridden".
-From Bonak Require Import SigT Notation RewLemmas HSet LeInductive.
+From Bonak Require Import SigT Notation RewLemmas HSet LeYoneda.
 
 Set Primitive Projections.
 Set Printing Projections.
 Set Keyed Unification.
+Set Typeclasses Depth 10.
 Remove Printing Let sigT.
 Remove Printing Let prod.
 
-(** The universe where the ν-parametric sets live *)
-Universe m.
-
-(** The universe where the type of ν-parametric sets live *)
-Universe m'.
-
 Section νType.
-(** The arity [ν] of parametric sets *)
 Variable arity: HSet.
 
-(**********************************************)
-(**
-A ν-parametric set is a family of sets obtained by iterating
-Reynolds' parametricity translation.
+Fixpoint FrameGen p: Type :=
+  match p with
+  | 0 => unit
+  | S p => { frames'': FrameGen p &T HSet }
+  end.
 
-For ν=1: this is a collection of colors, of points depending on a color,
-of lines connecting two points of the same color, of triangles filling a
-frame made of three connected lines, of tetrahedra filling a frame made
-of four glued triangles, etc.
-Intuitively, this is:
-  X₀ : hSet
-  (colors)
-  X₁ : X₀ → hSet
-  (points)
-  X₂ : Πx₀:X₀. X₁x₀ × X₁x₀ → hSet
-  (lines)
-  X₃ : Πx₀:X₀. Πy₀y₁y₂:X₁x₀. X₂x₀(y₀,y₁) × X₂x₀(y₀,y₂) × X₂x₀(y₁y₂) → hSet
-  (triangles)
-...
+Fixpoint PaintingGen p: FrameGen p -> Type :=
+  match p with
+  | 0 => fun _ => unit
+  | S p => fun frames'' => { painting'': PaintingGen p frames''.1 &T
+                             frames''.2 -> HSet }
+  end.
 
-Formally, following the recursive recipe defined in the file, this is
-equivalently defined as:
-  X₀ : unit → hSet                                                (colors)
-  X₁ : Σ⋆:unit.X₀⋆ → hSet                                         (points)
-  X₂ : Σx₁:(Σx₀:(Σ⋆:unit.X₀⋆).X₁x₀).X₁(x₁.1) → hSet               (lines)
-  X₃ : Σx₂':(Σx₂:(Σx₁':(Σx₁:(Σx₀:(Σ⋆:unit.X₀⋆).X₁x₀).X₁(x₁.1)).X₂(x₁')).
-              Σx₁:X₁(x₂.1.1).X₂(x₂.1,x₁)).
-        X₂((x₂'.1.1.1.1,x₂'.1.1.2),x₂'.2.1) → hSet                (triangles)
-
-  where each Xₙ has generically a type Xₙ : frameₙₙ(X₀,...,Xₙ₋₁) → hSet
-
-  Above, frameₙₙ has type pspₙ → hSet, where psp, standing for
-  "parametric set prefix", represents an initial sequence
-  X₀,...,Xₙ₋₁ of parametric sets.
-
-  Also, arguments of each Xᵢ in a frame are computed from previous arguments
-  using "restrictions". These restrictions themselves obey coherence rules.
-
-For ν=2: this is a collection of points, of lines connecting two points,
-of squares filling a frame made of four lines, of cubes filling a frame
-made of six squares, etc.
-Intuitively, this is:
-  X₀ : hSet
-  (points)
-  X₁ : X₀×X₀ → hSet
-  (lines)
-  X₂ : Πx₀₀x₀₁x₁₀x₁₁:X₀. X₁x₀₀x₁₀ × X₁x₁₀x₁₁ × X₁x₀₀x₀₁ × X₁x₁₀x₁₁ → hSet
-  (squares)
-
-Formally, it is built on a variant of frame that takes 2 copies of each X
-instead of 1.
-
-The construction mutually builds the type of frames, frame restrictions
-and coherence conditions on frame restrictions.
-*)
-
-Section RestrFramesDef.
-(** Assume what is needed to build restrFrameType and Frame(restrFrames)
-    at level n.+1 for respectively p < n and p <=  n.
-    In particular, n is here the level where live FramePrev and PaintingPrev. *)
-Variable n: nat.
-Variable FramePrev: forall p {Hp: p <~ n}, HSet.
-Variable PaintingPrev: forall p {Hp: p <~ n}, FramePrev p (Hp := Hp) -> HSet.
-
-Class RestrFrameTypeBlock := {
+Class RestrFrameTypeBlock p := {
   RestrFrameTypesDef: Type;
-  FrameDef: RestrFrameTypesDef -> HSet;
+  FrameDef: RestrFrameTypesDef -> FrameGen p.+1;
 }.
+
+Inductive ExtensionGen {p frames''} {paintings'': PaintingGen p frames''}:
+  forall {n: nat}, Type :=
+| TopPrev: ExtensionGen (n := 0)
+| AddExtraPrev {n: nat} {frame'': HSet} {painting'': frame'' -> HSet}:
+   ExtensionGen (p := p.+1) (frames'' := (frames''; frame''))
+     (paintings'' := (paintings''; painting'')) (n := n) ->
+   ExtensionGen (frames'' := frames'') (paintings'' := paintings'') (n := n.+1).
 
 (**
 Build the list of pairs of the type RestrFrameTypesDef(n+1,p) of
@@ -107,1431 +55,512 @@ That is, we build for p <= n.+1:
     frame_p(restrFrames_{0..p-1}) }
   n+1   : { restrFrameTypes = {RestrFrameType0 ... restrFrameType_n} ;
     frame(n+1,n+1)(restrFrames_{0..n})
+
+Example: if p = 0
+  RestrFrameTypesDef := []
+  FrameDef [] := [unit] (presented as a Sigma-type, i.e. as "unit")
 *)
-#[local]
-Instance mkRestrFrameTypesAndFrames:
-  forall p {Hp: p <~ n.+1}, RestrFrameTypeBlock :=
-  fix mkRestrFrameTypesAndFrames p:
-    forall (Hp: p <~ n.+1), RestrFrameTypeBlock :=
+Fixpoint mkRestrFrameTypesAndFrames' {p n}: forall
+  frames'' (paintings'': PaintingGen p frames''), RestrFrameTypeBlock p :=
   match p with
-  | O => fun (Hp: 0 <~ n.+1) =>
+  | 0 => fun frames'' paintings'' =>
     {|
       RestrFrameTypesDef := unit;
-      FrameDef _ := hunit
+      FrameDef _ := (tt; hunit) : FrameGen 1
     |}
-  | S p => fun (Hp: p.+1 <~ n.+1) =>
+  | p.+1 => fun frames'' paintings'' =>
+    let frames' := (mkRestrFrameTypesAndFrames' (n := n.+1) frames''.1 paintings''.1).(FrameDef) in
     {|
       RestrFrameTypesDef :=
-        { R: (mkRestrFrameTypesAndFrames p _).(RestrFrameTypesDef) &T
-          forall q (Hpq: p <~ q) (Hq: q <~ n) (ε: arity),
-          (mkRestrFrameTypesAndFrames p _).(FrameDef) R ->
-            FramePrev p (Hp := leI_lower_both Hp) };
+        { R: (mkRestrFrameTypesAndFrames' frames''.1 paintings''.1).(RestrFrameTypesDef) &T
+          forall q (Hq: q <= n) (ε: arity), (frames' R).2 -> frames''.2 };
       FrameDef R :=
-        { d: (mkRestrFrameTypesAndFrames p (leI_down Hp)).(FrameDef) R.1 &
-          hforall ε, PaintingPrev p (R.2 p (leI_refl _)
-             (leI_lower_both Hp) ε d) }
+        (frames' R.1; { d: (frames' R.1).2 & hforall ε, paintings''.2 (R.2 0 leY_O ε d) }) : FrameGen p.+2
     |}
   end.
 
-Definition mkRestrFrameTypes p {Hp: p <~ n.+1} :=
-  mkRestrFrameTypesAndFrames p (Hp := Hp).(RestrFrameTypesDef).
+Definition mkRestrFrameTypes' p n frames'' paintings'' :=
+  (mkRestrFrameTypesAndFrames' frames'' paintings'' (p := p)
+    (n := n)).(RestrFrameTypesDef).
 
-(** Additionally assume that we have restrFrames available up to level n
-    so as to build Frame and Painting at level n.+1 for any p <= n. *)
-Definition mkFullRestrFrameTypes :=
-  mkRestrFrameTypes n.+1 (Hp := leI_refl _).
-Variable FullRestrFrames: mkFullRestrFrameTypes.
-
-Definition restrictRestrFramesFromFull: forall p {Hp: p <~ n.+1},
-  mkRestrFrameTypes p :=
-  fix aux p Hp := match Hp with
-  | leI_refl _ => FullRestrFrames
-  | @leI_down _ p Hp => (aux p.+1 Hp).1
-  end.
-
-Definition mkFrameOfRestrFrames p {Hp: p <~ n.+1}:
-  mkRestrFrameTypes p (Hp := Hp) -> HSet :=
-  (mkRestrFrameTypesAndFrames p (Hp := Hp)).(FrameDef).
-
-(* Frame from full RestrFrames *)
-Definition mkFrame := fun p {Hp: p <~ n.+1} =>
-  mkFrameOfRestrFrames p (restrictRestrFramesFromFull p (Hp := Hp)).
-
-(* RestrFrame from full RestrFrames *)
-Definition mkRestrFrameFromFull p {Hp: p.+1 <~ n.+1} :=
-  (restrictRestrFramesFromFull p.+1 (Hp := Hp)).2:
-  forall q {Hpq: p <~ q} {Hq: q <~ n},
-    arity -> mkFrame p -> FramePrev p (Hp := leI_lower_both Hp).
-
-Definition mkPainting p {Hp: p <~ n.+1}
-  {E: mkFrame n.+1 -> HSet} := (fix aux p Hp :=
-  match Hp in p <~ _ return mkFrame p (Hp := Hp) -> HSet with
-  | leI_refl _ => E
-  | @leI_down _ p Hp => fun d =>
-       {l: hforall ε, PaintingPrev p (mkRestrFrameFromFull p p ε d) &
-        (aux p.+1 Hp) (d; l)}
-  end) p Hp.
-End RestrFramesDef.
-
-(** We build CohFrameType and RestrFrame at level n.+2 for respectively
-    p <= n and p <= n.+1, assuming:
-      - Frame'' and Painting'' for p <= n
-      - RestrFrames' for p <= n *)
-Section CohFramesDef.
-Variable n: nat.
-Variable Frame'': forall p {Hp: p <~ n}, HSet.
-Variable Painting'': forall p {Hp: p <~ n}, Frame'' p (Hp := Hp) -> HSet.
-Variable FullRestrFrames': mkFullRestrFrameTypes n Frame'' Painting''.
-Definition FrameFromFull' p {Hp: p <~ n.+1} :=
-  mkFrame n Frame'' Painting'' FullRestrFrames' p (Hp := Hp).
-Definition Frame' p {Hp: p <~ n.+1}
-  (r: mkRestrFrameTypes n Frame'' Painting'' p) :=
-  mkFrameOfRestrFrames n Frame'' Painting'' p (Hp := Hp) r.
-
-Definition RestrFrameFromFull'  p {Hp: p.+1 <~ n.+1} q {Hpq Hq} ε (d: FrameFromFull' p):
-  Frame'' p :=
-  mkRestrFrameFromFull n Frame'' Painting'' FullRestrFrames' p (Hp := Hp) q (Hpq := Hpq)
-  (Hq := Hq) ε d.
-Variable E': FrameFromFull' n.+1 (Hp := leI_refl _) -> HSet.
-Definition Painting' p {Hp: p <~ n.+1} :=
-  mkPainting n Frame'' Painting'' FullRestrFrames' p (Hp := Hp) (E := E').
-
-(** This is restrFrameType(n+2,0)..restrFrameType(n+2,p) for p <= n+1 *)
-Definition RestrFrameTypes p {Hp: p <~ n.+2}
-  (r: mkRestrFrameTypes n Frame'' Painting'' p) :=
-  mkRestrFrameTypes n.+1 (fun p Hp => Frame' r) Painting' p (Hp := Hp).
-
-Definition FrameOfRestrFrames p {Hp: p <~ n.+2}:
-  RestrFrameTypes p -> HSet :=
-  mkFrameOfRestrFrames n.+1 FrameFromFull' Painting' p (Hp := Hp).
-
-Class CohFrameTypeBlock p {Hp: p.+1 <~ n.+2}
-  (r: mkRestrFrameTypes n Frame'' Painting'' p (Hp := leI_lower_both Hp)) := {
-  CohFrameTypesDef: Type;
-  RestrFramesDef: CohFrameTypesDef -> RestrFrameTypes p.+1 (Hp := Hp);
-  (* up to RestrFrameType(n+2,p) *)
+Class FormDeps {p n} := {
+  _frames'': FrameGen p;
+  _paintings'': PaintingGen p _frames'';
+  _restrFrames': mkRestrFrameTypes' p n _frames'' _paintings'';
 }.
 
-Variable RestrPainting': forall p {Hp: p.+1 <~ n.+1} q {Hpq: p <~ q}
-  {Hq: q <~ n} ε (d: FrameFromFull' p),
-  Painting' (Hp := leI_down Hp) p d ->
-  Painting'' p (RestrFrameFromFull'  p q ε (Hpq := Hpq) (Hq := Hq) d).
+Arguments FormDeps p n: clear implicits.
+Generalizable Variables p n.
 
-(**
-Build the list of pairs of the type CohFrameType(n+2,p) of
-cohFrame(n+2,p) for p <= n and of the definition of restrFrame(n+2,p),
-for p <= n+1, in function of effective CohFrames of these types.
+Definition mkFrames' `(deps: FormDeps p n): FrameGen p.+1 :=
+  (mkRestrFrameTypesAndFrames' deps.(_frames'')
+    deps.(_paintings'') (n := n)).(FrameDef) deps.(_restrFrames').
 
-That is, we build for p <= n+1, where n is the level of Frame'':
-  p = 0 : { cohFrameTypes_{0..0-1} = unit ;
-   restrFrames(n+2,0)(cohFrames_{0..0-1}):restrFrameTypes_{0..0} }
-  p = 1 : { cohFrameTypes_{0..0} = {_:unit & cohFrameType(n+2,0)} ;
-   restrFrames_1(cohFrames_{0..0}):restrFrameTypes_{0..1} }
-  ...
-  p     : { cohFrameTypes_{0..p-1} = {_:unit & cohFrameType(n+2,0) ...
-   cohFrameType(n+2,p-1)} ;
-     restrFrames(n+2,p)(cohFrames_{0..p-1}):restrFrameTypes_{0..p} }
-  n+1   : { cohFrameTypes_{0..n} = {_:unit & cohFrameType(n+2,0) ...
-   cohFrameType(n+2,n)} ;
-     restrFrames(n+2,n+1)(cohFrames_{0..n}):restrFrameTypes_{0..n+1} }
-*)
+Definition mkFrame' `(deps: FormDeps p n): HSet :=
+  (mkFrames' deps).2.
+
+Class FormDep `(deps: FormDeps p n.+1) := {
+  _frame'': HSet;
+  _painting'': _frame'' -> HSet;
+  _restrFrame': forall q (Hq: q <= n) (ε: arity),
+    mkFrame' (n := n.+1) deps -> _frame''.(Dom);
+}.
+
+#[local]
+Instance ConsDep `(deps: FormDeps p n.+1)
+  (dep: FormDep deps): FormDeps p.+1 n :=
+{|
+  _frames'' := (deps.(_frames''); dep.(_frame'')): FrameGen p.+1;
+  _paintings'' := (deps.(_paintings''); dep.(_painting''));
+  _restrFrames' := (deps.(_restrFrames'); dep.(_restrFrame'));
+|}.
+
+#[local]
+Instance Proj1Deps `(deps: FormDeps p.+1 n): FormDeps p n.+1 := {|
+  _frames'' := deps.(_frames'').1;
+  _paintings'' := deps.(_paintings'').1;
+  _restrFrames' := deps.(_restrFrames').1;
+|}.
+
+#[local]
+Instance Proj2Deps `(deps: FormDeps p.+1 n): FormDep (Proj1Deps deps) := {|
+  _frame'' := deps.(_frames'').2;
+  _painting'' := deps.(_paintings'').2;
+  _restrFrame' := deps.(_restrFrames').2;
+|}.
+
+Declare Scope deps_scope.
+Delimit Scope deps_scope with deps.
+Bind Scope deps_scope with FormDeps.
+Notation "x .(1)" := (Proj1Deps x%_deps)
+  (at level 1, left associativity, format "x .(1)"): type_scope.
+Notation "x .(2)" := (Proj2Deps x%_deps)
+  (at level 1, left associativity, format "x .(2)"): type_scope.
+Notation "( x ; y )" := (ConsDep x y)
+  (at level 0, format "( x ; y )"): deps_scope.
+
+Inductive FormDepsExtension {p} : forall {n}, FormDeps p n -> Type :=
+| TopRestrFrames {deps}:
+  forall E': mkFrame' deps -> HSet,
+  FormDepsExtension (n := 0) deps
+| AddExtraRestrFrame {n} deps dep:
+  FormDepsExtension (ConsDep deps dep) ->
+  FormDepsExtension (n := n.+1) deps.
+
+Declare Scope extra_deps_scope.
+Delimit Scope extra_deps_scope with extradeps.
+Bind Scope extra_deps_scope with FormDepsExtension.
+Notation "( x ; y )" := (AddExtraRestrFrame _ x y)
+  (at level 0, format "( x ; y )"): extra_deps_scope.
+
+(* Example: if p := 0, extraDeps := ([],E')
+   mkPainting:= [E'] *)
+
+Fixpoint mkPainting' `{deps: FormDeps p n} (extraDeps: FormDepsExtension deps):
+  mkFrame' deps -> HSet :=
+  match extraDeps with
+  | TopRestrFrames E' => fun d => E' d
+  | AddExtraRestrFrame deps dep extraDeps => fun d =>
+      {l: hforall ε, dep.(_painting'') (dep.(_restrFrame') 0 leY_O ε d) &
+       mkPainting' extraDeps (d; l)}
+  end.
+
+Definition MatchPainting (loop: forall `{deps: FormDeps p n}
+  (extraDeps: FormDepsExtension deps),
+  PaintingGen p.+1 (mkFrames' deps)) {p n} :=
+  match p return forall `(deps: FormDeps p n)
+  (extraDeps: FormDepsExtension deps), PaintingGen p (mkFrames' deps).1 with
+  | 0 => fun _ _ => tt
+  | S p => fun deps extraDeps =>
+    loop (deps.(2); extraDeps)%extradeps
+  end.
+
+Fixpoint mkPaintings' `{deps: FormDeps p n}
+  (extraDeps: FormDepsExtension deps):
+  PaintingGen p.+1 (mkFrames' deps) :=
+  (MatchPainting (@mkPaintings') deps extraDeps; mkPainting' extraDeps).
+
+Lemma unfoldPaintingProj `{deps: FormDeps p n}
+  (extraDeps: FormDepsExtension deps) restrFrame:
+  (mkPaintings' extraDeps).2 restrFrame =
+    mkPainting' extraDeps restrFrame.
+Proof.
+  destruct p; now easy.
+Defined.
+
+(* Example: if p := 0, extraDeps := ([],E')
+   mkRestrFrameTypes := [unit -> unit] *)
+
+Definition mkRestrFrameTypes `(deps: FormDeps p n)
+  (extraDeps: FormDepsExtension deps) :=
+  (mkRestrFrameTypesAndFrames' (n := n) (mkFrames' deps)
+    (mkPaintings' extraDeps)).(RestrFrameTypesDef).
+
+Definition mkPrevRestrFrameTypes `(deps: FormDeps p n)
+  (extraDeps: FormDepsExtension deps) :=
+  (mkRestrFrameTypesAndFrames' (n := n.+1) (mkFrames' deps).1
+    (mkPaintings' extraDeps).1).(RestrFrameTypesDef).
+
+Definition mkDeps `{deps: FormDeps p n}
+  (extraDeps: FormDepsExtension deps)
+  (restrFrames: mkRestrFrameTypes deps extraDeps) :=
+{|
+  _frames'' := mkFrames' deps;
+  _paintings'' := mkPaintings' extraDeps;
+  _restrFrames' := restrFrames;
+|}.
+
+Definition mkFrame `{deps: FormDeps p n}
+  (extraDeps: FormDepsExtension deps)
+  (restrFrames: mkRestrFrameTypes deps extraDeps) :=
+  mkFrame' (mkDeps extraDeps restrFrames).
+
+Definition mkPrevFrame `{deps: FormDeps p n}
+  (extraDeps: FormDepsExtension deps)
+  (restrFrames: mkRestrFrameTypes deps extraDeps) :=
+  mkFrame' (mkDeps extraDeps restrFrames).(1).
+
+Class CohFrameTypeBlock `{deps: FormDeps p n}
+  {extraDeps: FormDepsExtension deps} := {
+  CohFrameTypesDef: Type;
+  RestrFramesDef: CohFrameTypesDef ->
+    mkRestrFrameTypes deps extraDeps
+}.
+
+Definition RestrPaintingType' `{deps: FormDeps p n.+1} (dep: FormDep deps)
+  (extraDeps: FormDepsExtension (deps; dep)) :=
+  forall q (Hq: q <= n) ε (d: mkFrame' deps),
+  mkPainting' (dep; extraDeps) d ->
+  dep.(_painting'') (dep.(_restrFrame') q Hq ε d).
+
+Fixpoint RestrPaintingTypes' {p}:
+  forall `{deps: FormDeps p n}
+  (extraDeps: FormDepsExtension deps), Type :=
+  match p with
+  | 0 => fun _ _ _ => unit
+  | S p =>
+    fun n deps extraDeps =>
+    { R: RestrPaintingTypes' (n := n.+1) (deps.(2); extraDeps) &T
+      RestrPaintingType' (p := p) deps.(2) extraDeps }
+  end.
+
 #[local]
 Instance mkCohFrameTypesAndRestrFrames:
-  forall p {Hp: p.+1 <~ n.+2} r, CohFrameTypeBlock p r :=
-  fix mkCohFrameTypesAndRestrFrames p:
-    forall (Hp: p.+1 <~ n.+2) (r: mkRestrFrameTypes n Frame'' Painting'' p (Hp := leI_lower_both Hp)), CohFrameTypeBlock p r :=
-  match p return forall Hp
-      (r: mkRestrFrameTypes n Frame'' Painting'' p (Hp := leI_lower_both Hp)), CohFrameTypeBlock p r with
-    | O => fun _ _ =>
+  forall `(deps: FormDeps p n)
+  (extraDeps: FormDepsExtension deps)
+  (restrPaintings': RestrPaintingTypes' extraDeps), CohFrameTypeBlock :=
+  fix mkCohFrameTypesAndRestrFrames {p}:
+  forall `(deps: FormDeps p n)
+    (extraDeps: FormDepsExtension deps)
+    (restrPaintings': RestrPaintingTypes' extraDeps), CohFrameTypeBlock :=
+  match p with
+  | 0 =>
+    fun n deps extraDeps restrPaintings' =>
     {|
       CohFrameTypesDef := unit;
-      RestrFramesDef _ := (tt; fun _ _ _ _ _ => tt): RestrFrameTypes 1
+      RestrFramesDef _ := (tt; fun _ _ _ _ => tt):
+        mkRestrFrameTypes deps extraDeps
     |}
-    | S p => fun (Hp: p.+2 <~ n.+2)
-        (restrFrames': mkRestrFrameTypes n Frame'' Painting'' p.+1 (Hp := leI_lower_both Hp)) =>
+  | S p =>
+    fun n deps extraDeps restrPaintings' =>
+    let restrFrames := (mkCohFrameTypesAndRestrFrames deps.(1)
+    (deps.(2); extraDeps)%extradeps restrPaintings'.1).(RestrFramesDef) in
+    let cohFrameTypes := (mkCohFrameTypesAndRestrFrames deps.(1)
+    (deps.(2); extraDeps)%extradeps restrPaintings'.1).(CohFrameTypesDef) in
     {|
-      CohFrameTypesDef := { Q:
-        (mkCohFrameTypesAndRestrFrames p (leI_down Hp) restrFrames'.1).(CohFrameTypesDef (Hp := leI_down Hp)) &T
+      CohFrameTypesDef := { Q: cohFrameTypes &T
         (* statement of cohFrameType(n+2,p) *)
-        forall r q (Hpq: p.+1 <~ q.+1) (Hpr: p.+1 <~ r.+1)
-          (Hrq: r.+1 <~ q.+1) (Hr: r.+1 <~ n.+1)
-          (Hq: q.+1 <~ n.+1) (ε ω: arity) d,
-        restrFrames'.2 p _ _ ε (*(leI_lower_both Hpq)
-          (leI_lower_both Hq) ε*)
-          (((mkCohFrameTypesAndRestrFrames p (leI_down Hp) restrFrames'.1).(RestrFramesDef
-            (Hp := leI_down Hp)) Q).2 r (leI_lower_both Hpr)
-            (leI_down Hr) ω d) =
-        restrFrames'.2 p (leI_lower_both Hp) r ω (leI_lower_both Hpr)
-          (leI_lower_both Hr)
-            (((mkCohFrameTypesAndRestrFrames p _).(RestrFramesDef) Q).2 q.+1
-              (leI_down Hpq) Hq ε d) };
+        forall r q (Hrq: r <= q) (Hq: q <= n) (ε ω: arity) d,
+        deps.(_restrFrames').2 q Hq ε
+          ((restrFrames Q).2 r (Hrq ↕ (↑ Hq)) ω d) =
+        deps.(_restrFrames').2 r (Hrq ↕ Hq) ω
+          ((restrFrames Q).2 q.+1 (⇑ Hq) ε d) };
       RestrFramesDef Q :=
       (* RestrFrame(n+2,p+1) *)
-      let restrFrame q := match q with
-      | O => fun (Hpq: p.+1 <~ 0) _ _ _ =>
-        False_rect _ (leI_O_contra Hpq)
-      | S q => fun (Hpq: p.+1 <~ q.+1) (Hq: q.+1 <~ n.+1) ε
-        (d: FrameOfRestrFrames p.+1 _) =>
-        (((mkCohFrameTypesAndRestrFrames p _).(RestrFramesDef) Q.1).2
-          q.+1 _ _ ε d.1 as rf in _;
-        fun ω => rew [Painting'' p] Q.2 p q Hpq (leI_refl _) Hpq
-          (leI_lower_both Hp) Hq ε ω d.1 in RestrPainting' p q ε _ (d.2 ω)
-          in forall ω, Painting'' p (RestrFrameFromFull'  _ _ _ rf))
-      end in ((mkCohFrameTypesAndRestrFrames p _).(RestrFramesDef) Q.1;
-        restrFrame): RestrFrameTypes p.+2
+      let restrFrame q (Hq: q <= n) ε
+        (d: mkFrame (deps.(2); extraDeps) (restrFrames Q.1)) :=
+          ((restrFrames Q.1).2 q.+1 (⇑ Hq) ε d.1 as rf in _;
+           fun ω => rew [deps.(_paintings'').2] Q.2 0 q leY_O Hq ε ω d.1 in
+            restrPaintings'.2 q _ ε _
+              (rew unfoldPaintingProj (deps.(2); extraDeps) _ in d.2 ω)
+           in forall ω,
+            deps.(_paintings'').2 (deps.(_restrFrames').2  _ _ _ rf))
+      in (restrFrames Q.1 as rf in _; restrFrame in forall q Hq ω,
+            (mkFrame (deps.(2); extraDeps)%extradeps rf) -> _)
+           : mkRestrFrameTypes deps extraDeps
     |}
   end.
 
-Definition mkCohFrameTypes p {Hp} :=
-  (mkCohFrameTypesAndRestrFrames p (Hp := Hp)).(CohFrameTypesDef).
+(* Example: if p := 0, extraDeps := ([],E')
+   mkCohFrameTypes := [] *)
 
-(** All CohFrameType(n+2,p) from p=0 to p=n *)
-Definition mkFullCohFrameTypes :=
-  mkCohFrameTypes n.+1 (Hp := leI_refl _).
+Definition mkCohFrameTypes `{deps: FormDeps p n}
+  {extraDeps: FormDepsExtension deps}
+  (restrPaintings': RestrPaintingTypes' extraDeps) :=
+  (mkCohFrameTypesAndRestrFrames deps extraDeps
+    restrPaintings').(CohFrameTypesDef).
 
-Variable FullCohFrames: mkFullCohFrameTypes.
+Definition mkRestrFrames `{deps: FormDeps p n}
+  {extraDeps: FormDepsExtension deps}
+  (restrPaintings': RestrPaintingTypes' extraDeps) :=
+  (mkCohFrameTypesAndRestrFrames deps extraDeps
+    restrPaintings').(RestrFramesDef).
 
-Definition mkRestrFramesFrom p {Hp} :=
-  (mkCohFrameTypesAndRestrFrames p (Hp := Hp)).(RestrFramesDef).
+Definition mkRestrFrame `{deps: FormDeps p n}
+  {extraDeps: FormDepsExtension deps}
+  (restrPaintings': RestrPaintingTypes' extraDeps) cohs:
+  forall q {Hq: q <= n} ε,
+    mkPrevFrame extraDeps (mkRestrFrames restrPaintings' cohs) ->
+    mkFrame' deps :=
+    (mkRestrFrames restrPaintings' cohs).2.
 
-(** All RestrFrame(n+2,p) from p=0 to p=n.+1 *)
-Definition mkFullRestrFrames :=
-  mkRestrFramesFrom n.+1 (Hp := leI_refl _) FullCohFrames.
+(* Example: if p := 0, extraDeps := ([],E'), restrPaintings' := , cohs := []
+   then mkFullDeps := {_frames'':=[unit];_paintings'':=[E']};_restrFrames':=[\qω().()]}
+   (where _restrFrames' is presented as a dependent pair, i.e. ((),\qω().()) *)
 
-(** Prefix of all CohFrame(n+2,i) from i=0 to i=p-1 *)
-Definition restrictCohFramesFromFull: forall p {Hp: p.+1 <~ n.+2},
-  mkCohFrameTypes p (Hp := Hp) :=
-  fix aux p (Hp: p.+1 <~ n.+2) :=
-  match Hp in S_p <~ _ return
-    match S_p return _ -> Type with 0 =>
-    fun _ => True | p.+1 => fun (Hp: p.+1 <~ n.+2) =>
-    mkCohFrameTypes p (Hp := Hp) end Hp with
-  | leI_refl _ => FullCohFrames
-  | @leI_down _ S_p Hp =>
-    match S_p return forall Hp',
-       match S_p return _ -> Type with 0 =>
-       fun _ => True | p.+1 => fun (Hp: p.+1 <~ n.+2) =>
-      mkCohFrameTypes p (Hp := Hp) end (leI_down Hp')
-    with 0 => fun _ => I | p.+1 => fun Hp => (aux p.+1 Hp).1 end Hp
+Definition mkFullDeps `{deps: FormDeps p n}
+  {extraDeps: FormDepsExtension deps}
+  (restrPaintings': RestrPaintingTypes' extraDeps)
+  (cohs: mkCohFrameTypes restrPaintings') :=
+  mkDeps extraDeps (mkRestrFrames restrPaintings' cohs).
+
+Definition mkCohFrameType `{deps: FormDeps p n.+1}
+  {dep: FormDep deps}
+  {extraDeps: FormDepsExtension (deps; dep)}
+  {restrPaintings': RestrPaintingTypes' (dep; extraDeps)}
+  (cohs: mkCohFrameTypes restrPaintings') :=
+  let restrFrame := (mkRestrFrames restrPaintings' cohs).2 in
+  forall r q (Hrq: r <= q) (Hq: q <= n) (ε ω: arity) d,
+      dep.(_restrFrame') q Hq ε (restrFrame r (Hrq ↕ (↑ Hq)) ω d)
+      = dep.(_restrFrame') r (Hrq ↕ Hq) ω (restrFrame q.+1 (⇑ Hq) ε d).
+
+Inductive CohFramesExtension {p}: forall `{deps: FormDeps p n}
+  {extraDeps: FormDepsExtension deps}
+  {restrPaintings': RestrPaintingTypes' extraDeps},
+  mkCohFrameTypes restrPaintings' -> Type :=
+| TopCoh
+    {deps}
+    {E': mkFrame' deps -> HSet}
+    {restrPaintings'}
+    {cohs: mkCohFrameTypes _}
+    {E: mkFrame _ (mkRestrFrames restrPaintings' cohs) -> HSet}
+    : CohFramesExtension (n := 0) (extraDeps := TopRestrFrames E') cohs
+| AddCohFrame {n deps dep extraDeps}
+    {restrPaintings': RestrPaintingTypes' (dep; extraDeps)}
+    {restrPainting': RestrPaintingType' dep extraDeps}
+    {cohs: mkCohFrameTypes restrPaintings'}
+    (coh: mkCohFrameType cohs):
+    CohFramesExtension (deps := (deps; dep))
+      (restrPaintings' := (restrPaintings'; restrPainting')) (cohs; coh) ->
+      CohFramesExtension (n := n.+1) (extraDeps := (dep; extraDeps)) cohs.
+
+Declare Scope extra_cohs_scope.
+Delimit Scope extra_cohs_scope with extracohs.
+Bind Scope extra_cohs_scope with CohFramesExtension.
+Notation "( x ; y )" := (AddCohFrame x y)
+  (at level 0, format "( x ; y )"): extra_cohs_scope.
+
+Fixpoint mkExtraDeps `{deps: FormDeps p n}
+  {extraDeps: FormDepsExtension deps}
+  {restrPaintings': RestrPaintingTypes' extraDeps}
+  {cohs: mkCohFrameTypes restrPaintings'}
+  (extraCohs: CohFramesExtension cohs):
+  FormDepsExtension (mkFullDeps restrPaintings' cohs).
+Proof.
+  destruct extraCohs.
+  - now constructor.
+  - unshelve econstructor.
+    + now apply (mkFullDeps (extraDeps := extraDeps)
+        (restrPaintings'; restrPainting') (cohs; coh)).(2).
+    + now apply (mkExtraDeps p.+1 n (deps; dep)%deps extraDeps
+        (restrPaintings'; restrPainting') (cohs; coh) extraCohs).
+Defined.
+
+Definition mkPainting `{deps: FormDeps p n}
+  {extraDeps: FormDepsExtension deps}
+  {restrPaintings': RestrPaintingTypes' extraDeps}
+  {cohs: mkCohFrameTypes restrPaintings'}
+  (extraCohs: CohFramesExtension cohs) :=
+  mkPainting' (mkExtraDeps extraCohs):
+  mkFrame (p := p) extraDeps _ -> HSet.
+
+Definition mkPrevPainting `{deps: FormDeps p n}
+  {extraDeps: FormDepsExtension deps}
+  {restrPaintings': RestrPaintingTypes' extraDeps}
+  {cohs: mkCohFrameTypes restrPaintings'}
+  (extraCohs: CohFramesExtension cohs) :=
+  mkPainting'
+    ((mkFullDeps restrPaintings' cohs).(2);
+      mkExtraDeps extraCohs)%extradeps:
+    mkPrevFrame (p := p) extraDeps (mkRestrFrames restrPaintings' cohs) -> HSet.
+
+Fixpoint mkRestrPainting `{deps: FormDeps p n}
+  {extraDeps: FormDepsExtension deps}
+  {restrPaintings': RestrPaintingTypes' extraDeps}
+  (cohs: mkCohFrameTypes restrPaintings')
+  (extraCohs: CohFramesExtension cohs):
+  forall q {Hq: q <= n} ε d, mkPrevPainting extraCohs d ->
+    mkPainting' extraDeps (mkRestrFrame restrPaintings' cohs q ε d).
+Proof.
+  intros * (l, c). destruct extraCohs, q.
+  - now apply (rew unfoldPaintingProj _ _ in l ε).
+  - exfalso. now apply leY_O_contra in Hq.
+  - now apply (rew unfoldPaintingProj _ _ in l ε).
+  - unshelve esplit.
+    + intro ω. rewrite <- coh with (Hrq := leY_O) (Hq := ⇓ Hq).
+      apply restrPainting'. simpl in l.
+      now apply (rew unfoldPaintingProj _ _ in l ω).
+    + now apply (mkRestrPainting _ _ _ extraDeps
+        (restrPaintings';restrPainting') (cohs; coh) _ q (⇓ Hq) ε
+        (d as x in _; l in _) c).
+Defined.
+
+Definition mkRestrPaintingTypes `{deps: FormDeps p n}
+  {extraDeps: FormDepsExtension deps}
+  {restrPaintings': RestrPaintingTypes' extraDeps}
+  (cohs: mkCohFrameTypes restrPaintings')
+  (extraCohs: CohFramesExtension cohs) :=
+  RestrPaintingTypes' (mkExtraDeps extraCohs).
+
+Fixpoint mkRestrPaintings `{deps: FormDeps p n}
+  {extraDeps: FormDepsExtension deps}
+  {restrPaintings': RestrPaintingTypes' extraDeps}
+  (cohs: mkCohFrameTypes restrPaintings')
+  (extraCohs: CohFramesExtension cohs):
+  mkRestrPaintingTypes cohs extraCohs.
+Proof.
+destruct p.
+  - unshelve esplit. now exact tt.
+    red; intros * c.
+    now eapply (mkRestrPainting cohs extraCohs q ε), c.
+  - unshelve esplit. now apply (mkRestrPaintings p n.+1 _ _ _ cohs.1
+      (cohs.2; extraCohs)%extracohs).
+    red; intros * c. now eapply (mkRestrPainting cohs extraCohs), c.
+Defined.
+
+Definition CohPaintingType `{deps: FormDeps p n.+1}
+  {dep: FormDep deps}
+  {extraDeps: FormDepsExtension (deps; dep)}
+  {restrPaintings': RestrPaintingTypes' (dep; extraDeps)}
+  {restrPainting': RestrPaintingType' dep extraDeps}
+  {cohs: mkCohFrameTypes restrPaintings'}
+  (coh: mkCohFrameType cohs)
+  (extraCohs: CohFramesExtension (deps := (deps; dep))
+    (restrPaintings' := (restrPaintings'; restrPainting'))
+    (cohs; coh)) :=
+  forall r q (Hrq: r <= q) (Hq: q <= n) (ε ω: arity) d c,
+  rew [dep.(_painting'')] coh r q Hrq Hq ε ω d in
+  restrPainting' q _ ε _ (mkRestrPainting cohs (coh; extraCohs) r ω d c) =
+  restrPainting' r _ ω _ (mkRestrPainting cohs (coh; extraCohs) q.+1 ε d c).
+
+Fixpoint CohPaintingTypes {p}:
+  forall `{deps: FormDeps p n}
+  {extraDeps: FormDepsExtension deps}
+  {restrPaintings': RestrPaintingTypes' extraDeps}
+  {cohs: mkCohFrameTypes restrPaintings'}
+  (extraCohs: CohFramesExtension cohs),
+  Type :=
+  match p with
+  | 0 => fun _ _ _ _ _ _ => unit
+  | S p =>
+    fun n deps extraDeps restrPaintings' cohs extraCohs =>
+    { R: CohPaintingTypes (cohs.2; extraCohs) &T
+         CohPaintingType cohs.2 extraCohs }
   end.
 
-
-(** RestrFrames(n+2,p) from full CohFrames, going down via RestrFrames *)
-Definition RestrFrames p {Hp: p.+1 <~ n.+2} :=
-  restrictRestrFramesFromFull n.+1 FrameFromFull' Painting' mkFullRestrFrames p.+1
-    (Hp := Hp).
-
-(** RestrFrames(n+2,p) from full CohFrames, going down via CohFrames *)
-Definition RestrFrames2 p {Hp: p.+1 <~ n.+2} :=
-  mkRestrFramesFrom p (Hp := Hp) (restrictCohFramesFromFull p (Hp := Hp)).
-
-Lemma eqRestrFramesDef {p} {Hp: p.+1 <~ n.+2}:
-  RestrFrames p (Hp := Hp) = RestrFrames2 p.
+Fixpoint mkCohFrames `{deps: FormDeps p n}
+  {extraDeps: FormDepsExtension deps}
+  {restrPaintings': RestrPaintingTypes' extraDeps}
+  (cohs: mkCohFrameTypes restrPaintings')
+  (extraCohs: CohFramesExtension cohs)
+  (cohPaintings: CohPaintingTypes extraCohs)
+  {struct p}:
+  mkCohFrameTypes (mkRestrPaintings cohs extraCohs).
 Proof.
-  induction Hp using leI_rectD. now easy. simpl in IHHp.
-  clear p; rename p0 into p. unfold RestrFrames, RestrFrames2 in *.
-  simpl. now rewrite IHHp.
-Defined.
-
-(** Frame(n+2,p) from full CohFrames, going down via RestrFrames *)
-Definition Frame p {Hp: p <~ n.+2} :=
-  mkFrame n.+1 FrameFromFull' Painting' mkFullRestrFrames p (Hp := Hp).
-
-(** Frame(n+2,p) from full CohFrames, going down via CohFrames *)
-Definition Frame2 p {Hp: p <~ n.+2} :=
-  FrameOfRestrFrames p
-    (match Hp in p <~ _ return (mkRestrFrameTypesAndFrames n.+1 FrameFromFull' Painting'
-      p).(RestrFrameTypesDef) with
-    | leI_refl _ => RestrFrames2 n.+1 (Hp := leI_refl _)
-    | @leI_down _ p Hp => (RestrFrames2 p (Hp := Hp)).1
-    end).
-
-Lemma eqFrameDef {p} {Hp: p <~ n.+2}:
-  Frame p (Hp := Hp) = Frame2 p (Hp := Hp).
-Proof.
-  destruct Hp. now easy.
-  now apply (f_equal (fun x =>
-    ((mkRestrFrameTypesAndFrames n.+1 FrameFromFull' Painting' p
-    (Hp := leI_down Hp)).(FrameDef)) x.1) (eqRestrFramesDef (Hp := Hp))).
-Defined.
-
-(** RestrFrame(n+2,p) from full CohFrames, going down via RestrFrames *)
-Definition RestrFrameFromFull p {Hp: p.+1 <~ n.+2} q {Hpq: p <~ q} {Hq: q <~ n.+1}
-  ε (d: Frame p): FrameFromFull' p (Hp := leI_lower_both Hp) :=
-  (RestrFrames p (Hp := Hp)).2 q Hpq Hq ε d.
-
-(** RestrFrame(n+2,p) from full CohFrames, going down via CohFrames *)
-Definition RestrFrame2 p {Hp: p.+1 <~ n.+2} q {Hpq: p <~ q} {Hq: q <~ n.+1}
-  ε (d: Frame2 p): FrameFromFull' p (Hp := leI_lower_both Hp) :=
-  (RestrFrames2 p (Hp := Hp)).2 q Hpq Hq ε d.
-
-Lemma eqRestrFrameDef {p} {Hp: p.+1 <~ n.+2} {q} {Hpq: p <~ q}
-  {Hq: q <~ n.+1} {ε} {d: Frame p}:
-  RestrFrameFromFull p q (Hpq := Hpq) (Hq := Hq) ε d =
-  RestrFrame2 p q (Hp := Hp) (Hpq := Hpq) (Hq := Hq) ε (rew eqFrameDef in d).
-Proof.
-  unfold RestrFrameFromFull, RestrFrame2, eqFrameDef.
-  rewrite <- rew_map with (f := fun x => (mkRestrFrameTypesAndFrames n.+1 Frame'
-      Painting' p (Hp := leI_down Hp)).(FrameDef) x.1).
-  now destruct eqRestrFramesDef.
-Defined.
-
-Definition CohFrame2 {p} {Hp: p.+2 <~ n.+2} r q {Hpq: p.+1 <~ q.+1}
-  {Hpr: p.+1 <~ r.+1} {Hrq: r.+1 <~ q.+1} {Hr: r.+1 <~ n.+1} {Hq: q.+1 <~ n.+1}
-  {ε ω: arity} (d: Frame2 p):
-  RestrFrameFromFull'  p q (Hpq := leI_lower_both Hpq)
-    (Hq := leI_lower_both Hq) ε (RestrFrame2 p r (Hp := leI_down Hp)
-      (Hpq := leI_lower_both Hpr) (Hq := leI_down Hr) ω d) =
-  RestrFrameFromFull'  p r (Hpq := leI_lower_both Hpr) (Hq := leI_lower_both Hr) ω
-    (RestrFrame2 p q.+1 (Hpq := leI_down Hpq) (Hq := Hq) ε d).
-Proof.
-  now exact ((restrictCohFramesFromFull p.+1).2 r q Hpq Hpr Hrq Hr Hq ε ω d).
-Defined.
-
-Definition CohFrame {p} {Hp: p.+2 <~ n.+2} r q {Hpq: p.+1 <~ q.+1}
-  {Hpr: p.+1 <~ r.+1} {Hrq: r.+1 <~ q.+1} {Hr: r.+1 <~ n.+1} {Hq: q.+1 <~ n.+1}
-  {ε ω: arity} (d: Frame p):
-  RestrFrameFromFull'  p q (Hpq := leI_lower_both Hpq)
-    (Hq := leI_lower_both Hq) ε (RestrFrameFromFull p r (Hp := leI_down Hp)
-      (Hpq := leI_lower_both Hpr) (Hq := leI_down Hr) ω d) =
-  RestrFrameFromFull'  p r (Hpq := leI_lower_both Hpr) (Hq := leI_lower_both Hr) ω
-    (RestrFrameFromFull p q.+1 (Hpq := leI_down Hpq) (Hq := Hq) ε d).
-Proof.
-  repeat rewrite eqRestrFrameDef.
-  now exact (CohFrame2 r q (rew eqFrameDef in d) (Hrq := Hrq)).
-Defined.
-
-Let coerceFrameSpType {p} {Hp: p.+1 <~ n.+2} := {d: Frame2 p &T
-  forall ε, Painting' p (RestrFrame2 p p (Hp := Hp)
-  (Hpq := leI_lower_both (leI_refl _)) (Hq := leI_lower_both Hp) ε d)} ->
-  Frame2 p.+1 (Hp := Hp).
-
-Definition coerceFrameSp {p} {Hp: p.+1 <~ n.+2}: coerceFrameSpType :=
-  match Hp in S_p <~ _ return
-    match S_p return _ -> Type with 0 =>
-    fun _ => True | p.+1 => fun (Hp: p.+1 <~ n.+2) =>
-      coerceFrameSpType (Hp := Hp) end Hp with
-  | leI_refl _ => id
-  | @leI_down _ S_p Hp =>
-      match S_p return forall Hp',
-       match S_p return _ -> Type with 0 =>
-       fun _ => True | p.+1 => fun (Hp: p.+1 <~ n.+2) =>
-        coerceFrameSpType (Hp := Hp) end (leI_down Hp')
-    with 0 => fun _ => I | p.+1 => fun Hp => id end Hp
-  end.
-
-Definition Painting2 p {Hp: p <~ n.+2} {E: Frame2 n.+2 -> HSet} :=
-  (fix aux p Hp :=
-  match Hp in p <~ _ return Frame2 (Hp := Hp) p -> HSet with
- | leI_refl _ => E
- | @leI_down _ p Hp => fun d =>
-    {l: hforall ε, Painting' p (RestrFrame2 p p ε d) &
-      (aux p.+1 Hp) (coerceFrameSp (d; l))}
-end) p Hp.
-
-Definition Painting p {Hp: p <~ n.+2} {E: Frame n.+2 -> HSet} :=
-  mkPainting n.+1 FrameFromFull' Painting' mkFullRestrFrames p (Hp := Hp) (E := E).
-
-Definition coercePaintingType {p} {Hp: p.+1 <~ n.+2}
-  {E: Frame n.+2 -> HSet} {d: Frame p}:
-  Painting p (Hp := leI_down Hp) (E := E) d ->
-  Painting2 p (Hp := leI_down Hp) (E := pi_domain_eq eqFrameDef E)
-    (rew eqFrameDef in d).
-Proof.
-  unfold Painting, Painting2; induction Hp using leI_rectD. now easy.
-  intros c. unshelve eapply existT.
-    - intros ε. rewrite <- eqRestrFrameDef. now apply c.1.
-    - set (l := c.2). apply IHHp in l. admit.
+destruct p.
+  - red; simpl. unshelve esplit. now exact tt. now intros.
+  - unshelve esplit.
+    + now apply (mkCohFrames p _ _ _ restrPaintings'.1 cohs.1
+      (cohs.2; extraCohs)%extracohs cohPaintings.1).
+    + intros. unshelve eapply eq_existT_curried.
+      * eapply ((mkCohFrames p _ _ _ restrPaintings'.1 cohs.1 (cohs.2; extraCohs)%extracohs cohPaintings.1).2 r.+1 q.+1 _ _ ε ω).
+      * (* prove a reorganization of the cohFrame using UIP *)
+        (* then: eapply (cohPaintings.2 r q _ _ ε ω). *)
 Admitted.
 
-Lemma RestrPainting2 p {Hp: p.+1 <~ n.+2} q {Hpq: p <~ q} {Hq: q <~ n.+1} ε
-  (d: Frame2 p) {E: Frame2 n.+2 -> HSet}:
-  Painting2 p (Hp := leI_down Hp) (E := E) d ->
-  Painting' p (RestrFrame2 p q (Hpq := Hpq) (Hq := Hq) ε d).
-Proof.
-  revert Hp Hq d.
-  induction Hpq using leI_invert.
-  - clear p q; rename n0 into p; intros Hp Hq.
-    replace Hq with (leI_lower_both Hp) by apply leI_irrelevance.
-    intros d c; now exact (c.1 ε).
-  - clear p q; rename p0 into p, n0 into q.
-    intros Hp Hq.
-    replace Hp with (leI_raise_both (leI_down (leI_trans Hpq Hq)))
-      by apply leI_irrelevance; clear Hp.
-    intros d c.
-    unshelve eapply existT. intros ω.
-    now exact (rew [Painting'' p]
-      CohFrame2 p q (Hpr := leI_refl _) (Hrq := Hpq) d in
-      RestrPainting' p q ε (RestrFrame2 p p ω d) (c.1 ω)).
-    set (l := c.2).
-    now apply (IHHpq (leI_raise_both (leI_trans Hpq Hq)) Hq _) in l.
-Defined.
+Definition mkExtraCohs `{deps: FormDeps p n}
+  {extraDeps: FormDepsExtension deps}
+  {restrPaintings': RestrPaintingTypes' extraDeps}
+  {cohs: mkCohFrameTypes restrPaintings'}
+  (extraCohs: CohFramesExtension cohs)
+  (cohPaintings: CohPaintingTypes extraCohs):
+  CohFramesExtension (mkCohFrames cohs extraCohs cohPaintings).
+Admitted.
 
-Lemma RestrPainting p {Hp: p.+1 <~ n.+2} q {Hpq: p <~ q} {Hq: q <~ n.+1} ε
-  (d: Frame p) {E: Frame n.+2 -> HSet}:
-  Painting p (Hp := leI_down Hp) (E := E) d ->
-  Painting' p (RestrFrameFromFull p q (Hpq := Hpq) (Hq := Hq) ε d).
-Proof.
-  intros Q; apply coercePaintingType in Q; rewrite eqRestrFrameDef; revert Q.
-  now exact (RestrPainting2 p q ε (rew eqFrameDef in d)
-    (E := pi_domain_eq eqFrameDef E)).
-Defined.
+Definition mkCohPaintings `{deps: FormDeps p n}
+  {extraDeps: FormDepsExtension deps}
+  {restrPaintings': RestrPaintingTypes' extraDeps}
+  (cohs: mkCohFrameTypes restrPaintings')
+  (extraCohs: CohFramesExtension cohs)
+  (cohPaintings: CohPaintingTypes extraCohs):
+  CohPaintingTypes (p := p.+1) (mkExtraCohs extraCohs cohPaintings).
+Admitted.
 
-End CohFramesDef.
-
-(** An ν-parametric type truncated at level [n] consists of:
-
-  - a [prefix] of parametric types up to dimension [n],
-  - a type of frames with their restrictions and coherence of
-    restrictions [Frame] (depending on their values are dimension [n]-1
-    and [n]-2) that are Σ-types of length [n] that is recursively built
-    out by induction on some [p] ranging from 0 to [n]
-  - a type of paintings (with their restrictions and coherence of
-    restrictions) [Painting] (depending on their values [PaintingPrev] at
-    dimensions [n]-1 and [n]-2) that are also recursively built out from
-    partial paintings
-  - axioms characterizing the definition of [Frame] and [Painting] in
-    the previous dimensions, so that the induction can be carried
-*)
-
-(** The construction maintains at each step of the induction the three
-    last levels of frames (called [frame''], [frame'], [frame]), the
-    two restrictions between them (called [restrFrame'] and
-    [restrFrame]) and the coherence between these two restrictions
-    (called [cohFrame]). *)
-
-(** We build paintings using an iterated construction: a painting at level n
-    depends on paintings at level n-1 and n-2; just as we have frame' and
-     frame'', we have painting' and painting''. *)
-
-Class νTypeAux n := {
-  frame'' p {Hp: p <~ n}: HSet;
-  painting'' p {Hp: p <~ n}: frame'' p -> HSet;
-  restrFrames': mkFullRestrFrameTypes n frame'' painting'';
-  frame' p {Hp: p <~ n.+1}: HSet :=
-    FrameFromFull' n frame'' painting'' restrFrames' p (Hp := Hp);
-  restrFrame' p {Hp: p.+1 <~ n.+1} q {Hpq Hq} ε (d: frame' p): frame'' p :=
-    RestrFrameFromFull'  n frame'' painting'' restrFrames' p
-    (Hp := Hp) q (Hpq := Hpq) (Hq := Hq) ε d;
-  painting' {E'} p {Hp: p <~ n.+1}: frame' p -> HSet :=
-    Painting' n frame'' painting'' restrFrames' E' p (Hp := Hp);
-  restrPainting' {E'} p {Hp: p.+1 <~ n.+1} q {Hpq: p <~ q} {Hq: q <~ n} ε
-    {d: frame' p}:
-    painting' (Hp := leI_down Hp) p d ->
-    painting'' p (restrFrame' p q ε (Hpq := Hpq) (Hq := Hq) d);
-  cohFrames {E'}:
-    mkFullCohFrameTypes n frame'' painting'' restrFrames' E' restrPainting';
-  restrFrames {E'}: mkFullRestrFrameTypes n.+1 frame' painting' :=
-    mkFullRestrFrames n frame'' painting'' restrFrames' E' restrPainting'
-    cohFrames;
-  frame {E'} p {Hp: p <~ n.+2}: HSet :=
-    Frame n frame'' painting'' restrFrames' E' restrPainting'
-    cohFrames p (Hp := Hp);
-  restrFrame {E'} p {Hp: p.+1 <~ n.+2} q {Hpq: p <~ q} {Hq: q <~ n.+1}
-    ε (d: frame p): frame' p :=
-    RestrFrameFromFull n frame'' painting'' restrFrames' E' restrPainting'
-    cohFrames p q ε d (Hp := Hp) (Hpq := Hpq) (Hq := Hq);
-  cohFrameType {E'} {p} {Hp: p.+2 <~ n.+2} {r q} {Hpq: p.+1 <~ q.+1}
-    {Hpr: p.+1 <~ r.+1} {Hrq: r.+1 <~ q.+1} {Hr: r.+1 <~ n.+1}
-    {Hq: q.+1 <~ n.+1} {ε ω d} :=
-    restrFrame' p q ε (restrFrame p r ω d
-      (Hp := leI_down Hp) (Hpq := leI_lower_both Hpr) (Hq := leI_down Hr)) =
-    restrFrame' p r ω (restrFrame p q.+1 ε d);
-  cohFrame {E'} {p} {Hp: p.+2 <~ n.+2} r q {Hpq: p.+1 <~ q.+1}
-    {Hpr Hrq Hr Hq} {ε ω} d:
-    cohFrameType (Hpq := Hpq) (Hrq := Hrq) :=
-    CohFrame n frame'' painting'' restrFrames' E' restrPainting'
-    cohFrames (Hp := Hp) (Hpr := Hpr) (Hrq := Hrq)
-    (Hr := Hr) (Hq := Hq) (ε := ε) (ω := ω) r q d;
-  painting {E'} p {Hp: p <~ n.+2} {E} (d: frame p): HSet :=
-    Painting n frame'' painting'' restrFrames' E'
-    restrPainting' cohFrames p d (Hp := Hp) (E := E);
-  restrPainting {E'} p {Hp: p.+1 <~ n.+2} q {Hpq: p <~ q} {Hq: q <~ n.+1}
-    ε {E} {d: frame p}:
-    painting p d -> painting' p (restrFrame p q ε d) :=
-    RestrPainting n frame'' painting'' restrFrames' E' restrPainting'
-    cohFrames p q ε (Hp := Hp) (Hpq := Hpq) (Hq := Hq) (E := E) d;
-  cohPainting {E'} {p} {Hp: p.+1 <~ n.+1} r q {Hpq: p.+1 <~ q.+1}
-    {Hpr: p.+2 <~ r.+2}
-    {Hrq: r <~ q} {Hr: r.+2 <~ n.+2} {Hq: q.+1 <~ n.+1} {ε ω E}
-    {d: frame p} (c: painting p d (E := E) (E' := E')
-      (Hp := leI_down (leI_down (leI_trans Hpr Hr)))):
-    rew [painting'' p] cohFrame r q d (Hpr := leI_lower_both Hpr)
-      (Hrq := leI_raise_both Hrq) in
-    restrPainting' p q ε (restrPainting p r ω c
-      (Hq := leI_down (leI_lower_both Hr))) =
-    restrPainting' p r ω (restrPainting p q.+1 ε c
-      (Hpq := leI_down Hpq) (Hq := Hq));
+Class νTypeAux p := {
+  deps: FormDeps p 0;
+  restrPaintings' E': RestrPaintingTypes' (TopRestrFrames E');
+  cohFrames E': mkCohFrameTypes (restrPaintings' E');
+  cohPaintings E' E: CohPaintingTypes (cohs := cohFrames E')
+    (TopCoh (E' := E') (E := E));
 }.
 
-(* We want ε and ω to be printed, but have them inferred;
-   Coq doesn't support this. *)
-
-Arguments frame'' {n} _ p {Hp}.
-Arguments painting'' {n} _ p {Hp} d.
-Arguments painting' {n} _ {E'} p {Hp} d.
-Arguments restrPainting' {n} _ {E'} p {Hp} q {Hpq Hq} ε [d] c.
-Arguments frame {n} _ {E'} p {Hp}.
-Arguments cohFrame {n} _ {E'} {p Hp} r q {Hpq Hpr Hrq Hr Hq ε ω}.
-Arguments painting {n} _ {E'} p {Hp E} d.
-Arguments restrPainting {n} _ {E'} p {Hp} q {Hpq Hq} ε {E} [d] c.
-Arguments cohPainting {n} _ {E'} {p Hp} r q {Hpq Hpr Hrq Hr Hq} {ε ω E} [d] c.
-
-Class νType n := {
-  prefix': Type;
-  data: prefix' -> νTypeAux n;
+Class νType p := {
+  prefix'': Type;
+  data: prefix'' -> νTypeAux p;
 }.
-
-Arguments prefix' {n} _.
 
 (***************************************************)
 (** The construction of [νType n+1] from [νType n] *)
 
 (** Extending the initial prefix *)
-Definition mkPrefix' {n} {C: νType n}: Type :=
-  { D: C.(prefix') &T (C.(data) D).(frame') n.+1 (Hp := leI_refl _) -> HSet }.
-
-(** The coherence conditions that Frame needs to satisfy to build the next level
-    of Frame. These will be used in the proof script of mkFrame. *)
+Definition mkPrefix'' p {C: νType p}: Type :=
+  { D: C.(prefix'') &T
+    mkFrame' (n := 0) (C.(data) D).(deps) -> HSet }.
 
 Section νTypeData.
-Variable n: nat.
-Variable C: νType n.
-Variable D: mkPrefix'.
+Variable p: nat.
+Variable C: νType p.
+Variable D: mkPrefix'' p.
 
-Definition mkFrame''' p {Hp: p <~ n} :=
-  (C.(data) D.1).(frame'') p (Hp := Hp).
+Definition mkDeps': FormDeps p.+1 0 :=
+  mkFullDeps _ ((C.(data) D.1).(cohFrames) D.2).
 
-Definition mkFrame'' p {Hp: p <~ n.+1} :=
-  (C.(data) D.1).(frame') p (Hp := Hp).
+Definition mkRestrPaintings' E': RestrPaintingTypes' _ :=
+  mkRestrPaintings
+  ((C.(data) D.1).(cohFrames) D.2) (TopCoh (E' := D.2) (E := E')).
 
-Definition mkFrame' p {Hp: p <~ n.+2} :=
-  (C.(data) D.1).(frame) p (Hp := Hp) (E' := D.2).
+Definition mkCohFrames' E': mkCohFrameTypes (mkRestrPaintings' E') :=
+  mkCohFrames ((C.(data) D.1).(cohFrames) D.2)
+   (TopCoh (E' := D.2) (E := E')) ((C.(data) D.1).(cohPaintings) D.2 E').
 
-Definition mkPainting''' p {Hp: p <~ n} :=
-  (C.(data) D.1).(painting'') p (Hp := Hp).
-
-Definition mkPainting'' p {Hp: p <~ n.+1} :=
-  (C.(data) D.1).(painting') p (Hp := Hp) (E' := D.2).
-
-Definition mkPainting' p {Hp: p <~ n.+2} {E} :=
-  (C.(data) D.1).(painting) p (Hp := Hp) (E' := D.2) (E := E).
-
-Definition mkRestrFrames'' :=
-  (C.(data) D.1).(restrFrames').
-
-Definition mkRestrFrames' :=
-  (C.(data) D.1).(restrFrames) (E' := D.2).
-
-Definition mkRestrFrame'' p {Hp: p.+1 <~ n.+1} q {Hpq: p <~ q} {Hq: q <~ n}
-  ε (d: mkFrame'' p) :=
-  (C.(data) D.1).(restrFrame') p q ε d (Hp := Hp) (Hpq := Hpq)
-    (Hq := Hq).
-
-Definition mkRestrFrame' p {Hp: p.+1 <~ n.+2} q {Hpq: p <~ q} {Hq: q <~ n.+1}
-  ε (d: mkFrame' p) :=
-  (C.(data) D.1).(restrFrame) (E' := D.2) p q ε d (Hp := Hp) (Hpq := Hpq)
-    (Hq := Hq).
-
-Definition mkRestrPainting'' p {Hp: p.+1 <~ n.+1} q {Hpq: p <~ q}
-  {Hq: q <~ n} ε: forall {d: mkFrame'' p},
-  mkPainting'' p d -> mkPainting''' p (mkRestrFrame'' p q ε
-    (Hp := Hp) (Hpq := Hpq) (Hq := Hq) d) :=
-  (C.(data) D.1).(restrPainting') p q ε (E' := D.2).
-
-Definition mkRestrPainting' {E'} p {Hp: p.+1 <~ n.+2} q {Hpq: p <~ q}
-  {Hq: q <~ n.+1} ε: forall {d: mkFrame' p},
-  mkPainting' p d -> mkPainting'' p (mkRestrFrame' p q ε
-    (Hp := Hp) (Hpq := Hpq) (Hq := Hq) d) :=
-  (C.(data) D.1).(restrPainting) p q ε (E' := D.2) (E := E').
-
-Definition mkCohFrames' :=
-  (C.(data) D.1).(cohFrames) (E' := D.2).
-
-Lemma CohRestrFramesAux : True.
-Admitted.
-
-Lemma CohFramesAux p (Hp: p.+1 <~ n.+2) RCF:
-  mkRestrFramesFrom n mkFrame''' mkPainting'''
-    mkRestrFrames'' D.2 mkRestrPainting'' p (Hp := Hp) RCF =
-  restrictRestrFramesFromFull n.+1 mkFrame'' mkPainting'' mkRestrFrames' p.+1
-    (Hp := Hp).
-Proof.
-  induction Hp using leI_rectD.
-  - unfold restrictRestrFramesFromFull, mkRestrFrames', mkFrame''', restrFrames.
-    unfold mkFullRestrFrames.
-    f_equal. admit.
-  - simpl. simpl in IHHp.
-    epose (RCF' := (RCF;_)).
-    now rewrite <- IHHp with (RCF := RCF').
-  Unshelve. simpl. intros.
-Admitted.
-(*
-Lemma EqRestrFrameDefAux {p} {Hp: p.+1 <~ n.+2} {q} {Hpq: p <~ q}
-  {Hq: q <~ n.+1} {ε} {d: Frame p}:
-  RestrFrameFromFull p q (Hpq := Hpq) (Hq := Hq) ε d =
-  RestrFrame2 p q (Hp := Hp) (Hpq := Hpq) (Hq := Hq) ε (rew eqFrameDef in d).
-*)
-(*
-Lemma eqRestrFramesDef' : mkRestrFrames' =
-  RestrFrames n mkFrame'' mkPainting'' mkRestrFrames' E' RestrPainting' FullCohFrames p0
-*)
-Definition mkCohFrames {E'}:
-  mkFullCohFrameTypes n.+1 mkFrame'' mkPainting'' mkRestrFrames' E'
-  mkRestrPainting'.
-Proof.
-unfold mkRestrFrames'. unfold restrFrames. unfold mkFullRestrFrames. unfold cohFrames.
-unfold mkFullCohFrameTypes. unfold mkCohFrameTypes.
-assert (forall p (Hp : p.+1 <~ n.+2),
-  mkCohFrameTypes n.+1 mkFrame'' mkPainting''
-(mkRestrFramesFrom n (C.(data) D.1).(frame'') (C.(data) D.1).(painting'') (C.(data) D.1).(restrFrames')
-     D.2 (C.(data) D.1).(restrPainting') p (restrictCohFramesFromFull _ _ _ _ _ _ _ _ (Hp:=Hp)))E'
-   mkRestrPainting' p.+1 (Hp := leI_raise_both Hp)).
-
- unfold mkRestrFramesFrom.
-change (mkRestrFramesFrom _ ?a ?b ?c ?d ?e _ _) with (RestrFrames2 _ a b c d e (C.(data) D.1).(cohFrames) n.+1 (Hp := leI_refl n.+2)).
-revert E'.
-rewrite <- (eqRestrFramesDef n (C.(data) D.1).(frame'') (C.(data) D.1).(painting'') (C.(data) D.1).(restrFrames') D.2
-     (C.(data) D.1).(restrPainting') (C.(data) D.1).(cohFrames) (Hp := leI_refl n.+2)).
-unfold mkRestrFramesFrom.
-red. unfold mkRestrFrames'. unfold restrFrames. unfold mkFullRestrFrames.
-  assert (forall p (Hp : p.+1 <~ n.+2),
-  mkCohFrameTypes n.+1 mkFrame'' mkPainting'' mkRestrFrames' E'
-   mkRestrPainting' p.+1 (Hp := leI_raise_both Hp)).
-  * induction p. simpl.
-    - intros Hp. unshelve eapply existT.
-      + now exact tt.
-      + intros. destruct d. unfold RestrFrameFromFull'.
-         change ((mkCohFrameTypesAndRestrFrames ?n ?a ?b ?c ?d ?e 0 (Hp:=?Hp)).(RestrFramesDef _ _ _ _ _) tt)
-           with (mkRestrFramesFrom n a b c d e 0 (Hp:=Hp) tt).
-simpl.
-unfold mkRestrFrameFromFull.
-         now rewrite <- CohFramesAux with
-            (Hp := (leI_lower_both (leI_raise_both Hp))) (RCF := tt).
-(*
-    - intros; exact tt.
-*)
-    - intros Hp. unshelve eapply existT.
-      + now exact (IHp (leI_down Hp)).
-      + intros.
-         change ((mkCohFrameTypesAndRestrFrames _ _ _ _ _ _ _).(RestrFramesDef _ _ _ _ _) ?CF)
-          with (mkRestrFramesFrom _ _ _ _ _ _ _ CF).
-         intros.
-unfold RestrFrameFromFull', mkRestrFrameFromFull.
-Arguments restrictRestrFramesFromFull n%nat_scope {FramePrev PaintingPrev FullRestrFrames} 
-  p%nat_scope Hp.
-destruct d as (d, l); simpl in d, l.
-        unfold mkRestrFramesFrom.
-        simpl ".2". destruct r.
-        ++ exfalso. now apply leI_lower_both, leI_O_contra in Hpr as [].
-        ++ simpl.
-            change ((mkCohFrameTypesAndRestrFrames _ _ _ _ _ _ _).(RestrFramesDef _ _ _ _ _) ?CF)
-             with (mkRestrFramesFrom _ _ _ _ _ _ _ CF).
-
-            rewrite <- CohFramesAux with (p:=p.+1) (Hp := (leI_lower_both (leI_raise_both Hp))). (RCF:=(IHp (leI_down Hp)).1).
-            admit.
-
-  * now exact (X n.+1 (leI_refl _)).
-Admitted.
-
-Let mkFrame {E'} p {Hp: p <~ n.+3} :=
-  Frame n.+1 mkFrame'' mkPainting'' mkRestrFrames' E' mkRestrPainting'
-  mkCohFrames p (Hp := Hp).
-
-Let mkRestrFrame {E'} p {Hp: p.+1 <~ n.+3} q {Hpq: p <~ q}
-  {Hq: q <~ n.+2} ε (d: mkFrame p) :=
-  RestrFrameFromFull n.+1 mkFrame'' mkPainting'' mkRestrFrames' E' mkRestrPainting'
-  mkCohFrames p q ε d (Hp := Hp) (Hpq := Hpq) (Hq := Hq).
-
-Let mkPainting {E'} p {Hp: p <~ n.+3} {E} (d: mkFrame p) :=
-  Painting n.+1 mkFrame'' mkPainting'' mkRestrFrames' E'
-  mkRestrPainting' mkCohFrames p d (Hp := Hp) (E := E).
-
-Definition mkRestrPainting {E'} p {Hp: p.+1 <~ n.+3} q {Hpq: p <~ q}
-  {Hq: q <~ n.+2} ε {E} {d: mkFrame p}:
-  mkPainting p d -> mkPainting' p (mkRestrFrame p q ε
-    (Hp := Hp) (Hpq := Hpq) (Hq := Hq) d) :=
-  RestrPainting n.+1 mkFrame'' mkPainting'' mkRestrFrames' E' mkRestrPainting'
-    mkCohFrames p q ε (Hp := Hp) (Hpq := Hpq) (Hq := Hq) (E := E) d.
-
-Definition mkCohFrame {E'} {p} {Hp: p.+2 <~ n.+3} r q {Hpq: p.+1 <~ q.+1}
-  {Hpr Hrq Hr Hq} {ε ω} (d: mkFrame p) :=
-  CohFrame n.+1 mkFrame'' mkPainting'' mkRestrFrames' E' mkRestrPainting'
-  mkCohFrames (Hp := Hp) (Hpq := Hpq) (Hpr := Hpr) (Hrq := Hrq)
-  (Hr := Hr) (Hq := Hq) (ε := ε) (ω := ω) r q d.
-
-Definition mkCohPainting {E'} {p} {Hp: p.+1 <~ n.+2} r q {Hpq: p.+1 <~ q.+1}
-  {Hpr: p.+2 <~ r.+2}
-  {Hrq: r <~ q} {Hr: r.+2 <~ n.+3} {Hq: q.+1 <~ n.+2} {ε ω E}
-  {d: mkFrame p} (c: mkPainting p d (E := E) (E' := E')
-  (Hp := leI_down (leI_down (leI_trans Hpr Hr)))): rew [mkPainting'' p] mkCohFrame r q d
-  (Hpr := leI_lower_both Hpr)
-  (Hrq := leI_raise_both Hrq) in
-  mkRestrPainting' p q ε (mkRestrPainting p r ω c
-  (Hq := leI_down (leI_lower_both Hr))) =
-  mkRestrPainting' p r ω (mkRestrPainting p q.+1 ε c
-  (Hpq := leI_down Hpq) (Hq := Hq)).
-Proof.
+Definition mkCohPaintings' E E': CohPaintingTypes (p := p.+1)
+  (cohs := mkCohFrames' E) (TopCoh (E := E')).
+(* Needs computation to typecheck
+  mkCohPaintings ((C.(data) D.1).(cohFrames) D.2)
+   (TopCoh (E' := _) (E := _)) ((C.(data) D.1).(cohPaintings) D.2 _). *)
 Admitted.
 
 End νTypeData.
 
 #[local]
-Instance mkνType {n} {C: νType n}: νType n.+1.
-Proof.
+Instance mkνType p {C: νType p}: νType p.+1.
   unshelve esplit.
-  now apply mkPrefix'.
-  unshelve esplit.
-  now eapply mkFrame''.
-  now eapply mkPainting''.
-  now eapply mkRestrFrames'.
-  now eapply mkRestrPainting'.
-  now eapply mkCohFrames.
-  now eapply mkCohPainting.
+  now exact (mkPrefix'' p).
+  intro D. unshelve esplit.
+  now eapply mkDeps'.
+  now apply mkRestrPaintings'.
+  now apply mkCohFrames'.
+  now apply mkCohPaintings'.
 Defined.
 
-Definition mkCohLayer {n} {C: νType n} {p r q} {Hpr: p.+3 <= r.+3}
-  {Hrq: r.+3 <= q.+3} {Hq: q.+3 <= n.+1} {ε ω}
-  {CF: CohFrameBlock n.+1 p mkPrefix mkFrame'' mkFrame' mkRestrFrameAux'}
-  {D} {d: CF.(RF).(Frame p) D} (l: mkLayer d):
-  rew [C.(layer')] CF.(CohFrame) r.+1 q.+1 d in
-    C.(restrLayer) p q ε (mkRestrLayer p r l) =
-    C.(restrLayer) p r ω (mkRestrLayer p q.+1 l).
-Proof.
-  intros *.
-  apply functional_extensionality_dep; intros 𝛉; unfold layer'.
-  rewrite <- map_subst_app with
-    (P := fun 𝛉 x => C.(painting'') (C.(restrFrame') p p 𝛉 x)).
-  unfold restrLayer, mkRestrLayer.
-  rewrite <- map_subst with (f := C.(restrPainting') p q ε).
-  rewrite <- map_subst with
-    (f := C.(restrPainting') p r ω).
-  rewrite rew_map with
-    (P := fun x => C.(painting'') x)
-    (f := fun x => C.(restrFrame') p p 𝛉 x),
-  rew_map with
-    (P := fun x => C.(painting'') x)
-    (f := fun x => C.(restrFrame') p q ε x),
-  rew_map with
-    (P := fun x => C.(painting'') x)
-    (f := fun x => C.(restrFrame') p r ω x).
-  rewrite <- (C.(cohPainting) p r q).
-  repeat rewrite rew_compose.
-  apply rew_swap with (P := fun x => C.(painting'') x).
-  rewrite rew_app_rl. now trivial.
-  now apply (C.(frame'') p D.1).(UIP).
-Qed.
-
-#[local]
-Instance mkCohFrameBlock0 {n} {C: νType n}:
-  CohFrameBlock n.+1 O mkPrefix mkFrame'' mkFrame' mkRestrFrameAux'.
-  unshelve esplit.
-  * unshelve esplit.
-    - intros. now exact hunit. (* Frame0 *)
-    - intros. now exact tt. (* restrFrame0 *)
-  * now intros.
-Defined.
-
-#[local]
-Instance mkCohFrameBlockSp {n} {C: νType n} {p}
-  {CF: CohFrameBlock n.+1 p mkPrefix mkFrame'' mkFrame' mkRestrFrameAux'}:
-  CohFrameBlock n.+1 p.+1 mkPrefix mkFrame'' mkFrame' mkRestrFrameAux'.
-  unshelve esplit.
-  * unshelve esplit.
-    - intros Hp D. now exact {d : CF.(RF).(Frame p) D & mkLayer d}.
-    - simpl; intros * ε * (d, l); invert_le Hpq. (* restrFramep *)
-      now exact (CF.(RF).(RestrFrame p) _ ε d; mkRestrLayer p q l).
-  * simpl; intros q r Hpr Hrq Hq ε ω D (d, l). (* cohframep *)
-    invert_le Hpr; invert_le Hrq.
-    now exact (= CF.(CohFrame) q.+1 r.+1 d; mkCohLayer l).
-Defined.
-
-(** Finally, we can define mkFrame at level n.+1 for all p *)
-#[local]
-Instance mkCohFrameBlock {n} {C: νType n} {p}:
-  CohFrameBlock n.+1 p mkPrefix mkFrame'' mkFrame' mkRestrFrameAux'.
-  induction p.
-  * now exact mkCohFrameBlock0. (* p = O *)
-  * now exact mkCohFrameBlockSp. (* p = S _ *)
-Defined.
-
-(** For [Painting], we take a different strategy. We first define [mkpainting],
-    [mkRestrPainting], and lemmas corresponding to their computational properties *)
-
-(** First, memoizing the previous levels of [Painting] *)
-Definition mkPainting'' {n} {C: νType n} {p} {Hp: p.+2 <= n.+1} {D: mkPrefix}:
-  mkFrame'' p D -> HSet := C.(painting').
-
-(** Then, the component [painting] of [Painting], built by upwards induction from [p] to [n] *)
-
-Definition mkPainting' {n} {C: νType n} {p} {Hp: p <= n.+1}
-  {D: mkPrefix} d: HSet := C.(painting) D.2 d.
-
-Definition mkPaintingType n {C: νType n} p {Hp: p <= n.+1} {D: mkPrefix}
-  (E: (mkCohFrameBlock).(RF).(Frame n.+1) D -> HSet)
-  (d: (mkCohFrameBlock).(RF).(Frame p) D): HSet :=
-  le_induction Hp (fun p Hp => mkCohFrameBlock.(RF).(Frame p) D -> HSet) E
-  (fun p Hp (Hind: mkCohFrameBlock.(RF).(Frame p.+1) (Hp := Hp) D -> HSet)
-    (d: mkCohFrameBlock.(RF).(Frame p) (Hp := ↓ Hp) D) =>
-    {l: mkLayer d & Hind (d; l)}) d.
-
-Lemma mkPaintingType_base_computes {n} {C: νType n}
-  {D E} {d: (mkCohFrameBlock).(RF).(Frame n.+1) D}:
-  mkPaintingType n n.+1 E d = E d.
-Proof.
-  unfold mkPaintingType; now rewrite le_induction_base_computes.
-Qed.
-
-Lemma mkPaintingType_step_computes {n p} {C: νType n} {Hp: p.+1 <= n.+1} {D}
-  {E: (mkCohFrameBlock).(RF).(Frame n.+1) D -> HSet} {d}:
-  mkPaintingType n p E d =
-  {l: mkLayer d & mkPaintingType n p.+1 E (d; l)} :> Type.
-Proof.
-  unfold mkPaintingType; now rewrite le_induction_step_computes.
-Qed.
-
-(** Now, [restrPainting], and the corresponding computational properties. *)
-
-Definition mkRestrPainting {n} {C: νType n} p q {Hpq: p.+1 <= q.+1}
-  {Hq: q.+1 <= n.+1} {ε} {D} E (d: (mkCohFrameBlock).(RF).(Frame p) D)
-  (c: mkPaintingType n p E d):
-  mkPainting' ((mkCohFrameBlock).(RF).(RestrFrame p) q ε d).
-Proof.
-  revert d c; simpl. apply le_induction' with (Hp := Hpq).
-  * intros d c. destruct (rew [id] mkPaintingType_step_computes in c) as (l, _).
-    now exact (l ε).
-  * clear p Hpq; intros p Hpq mkRestrPaintingSp d c; invert_le Hpq.
-    destruct (rew [id] mkPaintingType_step_computes in c) as (l, c'). clear c.
-    rewrite C.(eqPaintingSp). apply mkRestrPaintingSp in c'.
-    now exact (mkRestrLayer p q l; c').
-Defined.
-
-Lemma mkRestrPainting_base_computes {n} {C: νType n} {p} {Hp: p.+1 <= n.+1}
-  {ε} {D E} {d: (mkFrame p).(frame p) D} {c}:
-  mkRestrPainting p p E d c =
-  match (rew [id] mkPaintingType_step_computes in c) with
-  | (l; _) => l ε
-  end.
-Proof.
-  unfold mkRestrPainting; now rewrite le_induction'_base_computes.
-Qed.
-
-Lemma mkRestrPainting_step_computes {n} {C: νType n} {r q} {Hrq: r.+2 <= q.+2}
-  {Hq: q.+2 <= n.+1} {ε} {D E} {d: (mkFrame r).(frame r) D} {c}:
-  mkRestrPainting r q.+1 (Hpq := ↓ Hrq) (Hq := Hq) (ε := ε) E d c =
-  match (rew [id] mkPaintingType_step_computes in c) with
-  | (l; c) => rew <- [id] C.(eqPaintingSp) in
-      (mkRestrLayer r q l; mkRestrPainting r.+1 q.+1 E (d; l) c)
-  end.
-Proof.
-  unfold mkRestrPainting; now rewrite le_induction'_step_computes.
-Qed.
-
-(** Now, for the last part of the proof: proving coherence conditions
-    on [cohPainting] *)
-
-(** The base case is easily discharged *)
-Definition mkCohPainting_base {n} {C: νType n} {r q}
-  {Hrq: r.+2 <= q.+2} {Hq: q.+2 <= n.+1} {ε ω}
-  {D} {E: (mkFrame n.+1).(frame n.+1) D -> HSet}
-  (d: (mkFrame r).(frame r) D) (c: mkPaintingType n r E d):
-  rew [mkPaintingPrev.(painting'')] (mkFrame r).(cohFrame) r q d in
-    mkPaintingPrev.(restrPainting') r q ε
-      (mkRestrPainting r r (ε := ω) E d c) =
-  mkPaintingPrev.(restrPainting') r r ω
-    (mkRestrPainting r q.+1 (ε := ε) E d c).
-Proof.
-  rewrite mkRestrPainting_base_computes, mkRestrPainting_step_computes.
-  destruct (rew [id] mkPaintingType_step_computes in c) as (l, c'); clear c.
-  now exact (C.(eqRestrPainting0) (mkRestrPainting r.+1 q.+1 E (_; _) c')).
-Qed.
-
-(** A small abbreviation *)
-Definition mkCohPaintingHyp {n} {C: νType n}
-  p r q {Hpr: p.+2 <= r.+3} {Hrq: r.+3 <= q.+3} {Hq: q.+3 <= n.+1}
-  ε ω {D} {E: (mkFrame n.+1).(frame n.+1) D -> HSet}
-  {d: (mkFrame p).(frame p) D}
-  (c: mkPaintingType n p E d) :=
-  rew [mkPaintingPrev.(painting'')] (mkFrame p).(cohFrame) r.+1 q.+1 d in
-  C.(Painting).(restrPainting) p q.+1 (ε := ε)
-    (mkRestrPainting p r.+1 E d c) =
-  C.(Painting).(restrPainting) p r.+1 (ε := ω)
-    (mkRestrPainting p q.+2 (ε := ε) E d c).
-
-(** The step case is discharged as (mkCohLayer; IHP) *)
-Definition mkCohPainting_step {n} {C: νType n} {p r q} {Hpr: p.+3 <= r.+3}
-  {Hrq: r.+3 <= q.+3} {Hq: q.+3 <= n.+1} {ε ω}
-  {D} {E: (mkFrame n.+1).(frame n.+1) D -> HSet}
-  {d: (mkFrame p).(frame p) D} {c: mkPaintingType n p E d}
-  {IHP: forall (d: (mkFrame p.+1).(frame p.+1) D)
-        (c: mkPaintingType n p.+1 E d), mkCohPaintingHyp p.+1 r q ε ω c}:
-        mkCohPaintingHyp p r q ε ω c.
-Proof.
-  unfold mkCohPaintingHyp in *.
-  do 2 rewrite mkRestrPainting_step_computes.
-  destruct (rew [id] mkPaintingType_step_computes in c) as (l, c'); clear c.
-  rewrite (C.(eqRestrPaintingSp) p q), (C.(eqRestrPaintingSp) p r).
-  rewrite <- rew_permute_rl with (H := C.(@eqPaintingSp' _) _ _ _).
-  f_equal.
-  unshelve eapply (rew_existT_curried
-    (Q := fun x =>
-      C.(PaintingPrev).(painting') (rew <- [id] C.(eqFrameSp') in x))).
-  - now exact (mkCohLayer l).
-  - rewrite <- IHP with (d := (d; l)) (c := c').
-    simpl (mkFrame p.+1). unfold mkPaintingPrev, painting''.
-    unfold mkFrameSp, cohFrame.
-    rewrite rew_map with (P := fun x => C.(PaintingPrev).(painting') x)
-                       (f := fun x => rew <- [id] C.(eqFrameSp') in x).
-    repeat rewrite rew_compose.
-    repeat rewrite <- eq_trans_assoc.
-    now rewrite eq_trans_sym_inv_l, eq_trans_refl_r.
-Qed.
-
-(** Build a [PaintingBlock n.+1] using what we just defined *)
-#[local]
-Instance mkPainting {n} {C: νType n}:
-  PaintingBlock n.+1 mkPrefix mkPaintingPrev mkFrame.
-  unshelve esplit; intros p.
-  * intros *; now apply mkPaintingType.
-  * intros q Hpq Hq ε d; now exact (mkRestrPainting p q).
-  * intros *. revert d c. pattern p, Hpr. apply le_induction''.
-    + now exact mkCohPainting_base.
-    + clear p Hpr; unfold mkPaintingPrev, restrPainting'; cbv beta iota;
-      intros p Hpr IHP d c; invert_le Hpr; invert_le Hrq.
-      now exact (mkCohPainting_step (IHP := IHP)).
-Defined.
-
-(** The base case of a ν-parametric set (truncated at dimension 0) *)
-
-#[local]
-Instance mkνType0: νType 0.
-  unshelve esplit.
-  - now exact hunit.
-  - unshelve esplit.
-    * intros; now le_contra Hp.
-    * intros; now le_contra Hp.
-    * intros;now le_contra Hq.
-  - unshelve esplit.
-    * intros Hp _; now exact hunit.
-    * intros; now le_contra Hq.
-    * intros; now le_contra Hq.
-  - unshelve esplit; intros.
-    * now le_contra Hp.
-    * now le_contra Hp.
-    * now le_contra Hq.
-  - unshelve esplit.
-    * intros p Hp D E d. now exact (E d).
-    * intros; now le_contra Hq.
-    * intros; now le_contra Hq.
-  - now intros.
-  - intros; now le_contra len1.
-  - intros; now le_contra Hp.
-  - intros; now le_contra Hp.
-  - intros; now le_contra Hq.
-  - intros; now le_contra Hp.
-  - intros; now le_contra Hp.
-  - intros; now le_contra Hq.
-  - intros; now le_contra Hp.
-  - intros; now le_contra Hq.
-Defined.
-
-(** We are now ready to build an [νType n.+1] from an [νType n] *)
-#[local]
-Instance mkνTypeSn {n} (C: νType n): νType n.+1 :=
-{|
-    prefix := mkPrefix;
-    FramePrev := mkFramePrev;
-    Frame := mkFrame;
-    PaintingPrev := mkPaintingPrev;
-    Painting := mkPainting;
-    eqFrame0 := ltac:(now intros *);
-    eqFrame0' := ltac:(intros *; now apply C.(eqFrame0));
-    eqFrameSp := ltac:(now intros *);
-    eqFrameSp' := ltac:(intros *; now apply C.(eqFrameSp));
-    eqRestrFrame0 := ltac:(now intros *);
-    eqRestrFrameSp := ltac:(now intros *);
-    eqPaintingSp := ltac:(intros *; now apply mkPaintingType_step_computes);
-    eqPaintingSp' := ltac:(intros *; now apply C.(eqPaintingSp));
-    eqRestrPainting0 := ltac:(intros *; simpl;
-      now rewrite mkRestrPainting_base_computes, rew_rew');
-    eqRestrPaintingSp := ltac:(intros *; simpl;
-      now rewrite mkRestrPainting_step_computes, rew_rew');
-|}.
-
-(** An [νType] truncated up to dimension [n] *)
-Fixpoint νTypeAt n: νType n :=
-  match n with
-  | O => mkνType0
-  | n.+1 => mkνTypeSn (νTypeAt n)
-  end.
-
-(** The coinductive suffix of an [νType] beyond level [n] *)
-CoInductive νTypeFrom n (X: (νTypeAt n).(prefix)): Type@{m'} := cons {
-  this: (νTypeAt n).(Frame).(frame n) X -> HSet;
-  next: νTypeFrom n.+1 (X; this);
-}.
-
-Arguments this {n X} _ d.
-Arguments next {n X} _.
-
-(** The final construction *)
-Definition νTypes := νTypeFrom 0 tt.
-
-(** Degeneracies *)
-
-Class mkRefl T := intro_mkrefl : T -> Type@{m'}.
-Class mk {T} (f: T -> Type@{m'}) (t: T) := intro_mk : f t.
-
-Class DgnFrameBlockPrev {n'} (C: νType n'.+1)
-  {reflPrefix: mkRefl C.(prefix)} := {
-  reflFrame' p {Hp: p.+2 <= n'.+1} {D} {R: mk reflPrefix D}:
-    C.(FramePrev).(frame'') p D -> C.(FramePrev).(Frames) p D;
-}.
-
-Arguments reflFrame' {n' C reflPrefix} _ p {Hp D R} d.
-
-Class DgnFrameBlock {n'} (C: νType n'.+1) {reflPrefix: mkRefl C.(prefix)}
-  p (Prev: DgnFrameBlockPrev C) := {
-  reflFrame {Hp: p.+1 <= n'.+1} {D} {R: mk reflPrefix D}:
-    C.(FramePrev).(Frames) p D -> C.(Frame).(frame p) D;
-  idReflRestrFrame {ε} {Hp: p.+1 <= n'.+1} {D} {R: mk reflPrefix D}
-    {d: C.(FramePrev).(Frames) p D}:
-    C.(Frame).(restrFrame) n' ε (reflFrame d) = d;
-  cohReflRestrFrame q {ε} {Hpq: p.+2 <= q.+2} {Hq: q.+2 <= n'.+1} {D}
-    {R: mk reflPrefix D} {d: C.(FramePrev).(Frames) p D}:
-    Prev.(reflFrame') p (C.(FramePrev).(restrFrame') p q ε d) =
-      C.(Frame).(restrFrame) q ε (reflFrame d);
-}.
-
-Arguments reflFrame {n' C reflPrefix p Prev} _ {Hp D R} d.
-Arguments idReflRestrFrame {n' C reflPrefix p Prev} _ {ε Hp D R d}.
-Arguments cohReflRestrFrame {n' C reflPrefix p Prev} _ q {ε Hpq Hq D R d}.
-
-Class DgnPaintingBlockPrev {n'} (C: νType n'.+1) {reflPrefix: mkRefl C.(prefix)}
-  (Prev: DgnFrameBlockPrev C) := {
-  reflPainting' p {Hp: p.+2 <= n'.+1} {D} {R: mk reflPrefix D}
-    {d: C.(FramePrev).(frame'') p D}:
-    C.(PaintingPrev).(painting'') d ->
-    C.(PaintingPrev).(painting') (Prev.(reflFrame') p d);
-}.
-
-Arguments reflPainting' {n' C reflPrefix Prev} _ p {Hp D R d} c.
-
-Class HasRefl {n'} {C: νType n'.+1} {reflPrefix: mkRefl C.(prefix)}
-  {DgnFramePrev: DgnFrameBlockPrev C}
-  {DgnFrame: forall {p}, DgnFrameBlock C p DgnFramePrev} {D}
-  {R: mk reflPrefix D} (E: _ -> HSet) :=
-  hasRefl: forall (d: C.(FramePrev).(Frames) n' D)
-    (c: C.(PaintingPrev).(painting') d),
-    let l ε :=
-      rew <- [C.(PaintingPrev).(painting')] DgnFrame.(idReflRestrFrame) in c in
-     E (rew <- [id] C.(eqFrameSp) in (DgnFrame.(reflFrame) d; l)).
-
-Class DgnPaintingBlock {n'} (C: νType n'.+1) {reflPrefix: mkRefl C.(prefix)}
-  {Q: DgnFrameBlockPrev C}
-  (Prev: DgnPaintingBlockPrev C Q)
-  (FrameBlock: forall {p}, DgnFrameBlock C p Q) := {
-  reflPainting p {Hp: p.+1 <= n'.+1} {D} {R: mk reflPrefix D} {E}
-    {L: HasRefl E} {d: C.(FramePrev).(Frames) p D}:
-    C.(PaintingPrev).(painting') d ->
-    C.(Painting).(painting) E (FrameBlock.(reflFrame) d);
-  idReflRestrPainting {p ε} {Hp: p.+1 <= n'.+1} {D} {R: mk reflPrefix D}
-    {E} {L: HasRefl E}
-    {d: C.(FramePrev).(Frames) p D} {c: C.(PaintingPrev).(painting') d}:
-    rew [C.(PaintingPrev).(painting')] FrameBlock.(idReflRestrFrame) in
-    C.(Painting).(restrPainting) p n' (ε := ε) (E := E) (reflPainting p c) = c;
-  cohReflRestrPainting {p} q {ε} {Hpq: p.+2 <= q.+2} {Hq: q.+2 <= n'.+1} {D}
-    {R: mk reflPrefix D} {E} {L: HasRefl E} {d: C.(FramePrev).(Frames) p D}
-    {c: C.(PaintingPrev).(painting') d}:
-    rew <- [C.(PaintingPrev).(painting')] FrameBlock.(cohReflRestrFrame) q in
-    C.(Painting).(restrPainting) p q (ε := ε) (E := E) (reflPainting p c) =
-    Prev.(reflPainting') p (C.(PaintingPrev).(restrPainting') _ q ε c);
-}.
-
-Arguments reflPainting {n' C reflPrefix Q Prev FrameBlock} _ p {Hp D R E L d} c.
-Arguments idReflRestrPainting {n' C reflPrefix Q Prev FrameBlock} _ {p ε Hp D R
-  E L d c}.
-Arguments cohReflRestrPainting {n' C reflPrefix Q Prev FrameBlock} _ {p} q
-  {ε Hpq Hq D R E L d c}.
-
-(** Dgn is the extra structure to support degeneracies, which we call Refl *)
-
-Class Dgn {n'} (C: νType n'.+1) := {
-  ReflPrefix: mkRefl C.(prefix);
-  DgnFramePrev: DgnFrameBlockPrev C;
-  DgnFrame {p}: DgnFrameBlock C p DgnFramePrev;
-  DgnPaintingPrev: DgnPaintingBlockPrev C DgnFramePrev;
-  DgnPainting: DgnPaintingBlock C DgnPaintingPrev (@DgnFrame);
-  ReflLayer {p} {Hp: p.+2 <= n'.+1} {D} {R: mk ReflPrefix D}
-    {d: C.(FramePrev).(Frames) p D}
-    (l: C.(layer') d): C.(Layer) (DgnFrame.(reflFrame) d) :=
-    fun ε => rew [C.(PaintingPrev).(painting')]
-    DgnFrame.(cohReflRestrFrame) p in DgnPaintingPrev.(reflPainting') p (l ε);
-  eqReflFrameSp {p q} {Hpq: p.+2 <= q.+2} {Hq: q.+2 <= n'.+1} {D}
-    {R: mk ReflPrefix D} {d: C.(FramePrev).(Frames) p D} (l: C.(layer') d):
-    DgnFrame.(reflFrame) (rew <- [id] C.(eqFrameSp') in (d; l)) =
-    rew <- [id] C.(eqFrameSp) in (DgnFrame.(reflFrame) d; ReflLayer l);
-  eqReflPaintingSp p q {Hpq: p.+2 <= q.+2} {Hq: q.+2 <= n'.+1} {D}
-    {R: mk ReflPrefix D} {E} {L: HasRefl E} {d} {l: C.(layer') d}
-    {c: C.(PaintingPrev).(painting') (D := D)
-      (rew <- [id] C.(eqFrameSp') in (d; l))}:
-    DgnPainting.(reflPainting) p (rew <- [id] C.(eqPaintingSp') in (l; c)) =
-    rew <- [id] C.(eqPaintingSp) in
-      (ReflLayer l; rew [C.(Painting).(painting) E] eqReflFrameSp l in
-        DgnPainting.(reflPainting) p.+1 c);
-}.
-
-Arguments ReflPrefix {n' C} _.
-Arguments DgnFramePrev {n' C} _.
-Arguments DgnFrame {n' C} _ {p}.
-Arguments DgnPaintingPrev {n' C} _.
-Arguments DgnPainting {n' C} _.
-Arguments ReflLayer {n' C} _ {p Hp D R d} l.
-Arguments eqReflFrameSp {n' C} _ {p q Hpq Hq D R d} l.
-Arguments eqReflPaintingSp {n' C} _ p q {Hpq Hq D R E L d l c}.
-
-#[local]
-Instance mkReflPrefix {n'} {C: νType n'.+1} {G: Dgn C}: mkRefl
-  (mkνTypeSn C).(prefix) :=
-  fun D => { R : mk G.(ReflPrefix) D.1 &_T
-  HasRefl (DgnFrame := fun p => G.(DgnFrame)) D.2 }.
-
-#[local]
-Instance mkDgnFramePrev {n'} {C: νType n'.+1} {G: Dgn C}:
-  DgnFrameBlockPrev (mkνTypeSn C) := {|
-  reflFrame' p Hp (D: (mkνTypeSn C).(prefix)) R :=
-    G.(DgnFrame).(reflFrame) (R := R.1);
-|}.
-
-Definition mkReflLayer {n' p} {C: νType n'.+1} {G: Dgn C}
-  {Hp: p.+2 <= n'.+2} {Frame: DgnFrameBlock (mkνTypeSn C) p mkDgnFramePrev}
-  {D} {R: mk mkReflPrefix D} {d: mkFramePrev.(Frames) p D} (l: mklayer' d):
-  mkLayer (Frame.(reflFrame) d) :=
-  fun ω => rew [C.(Painting).(painting) D.2]
-    Frame.(cohReflRestrFrame) p in G.(DgnPainting).(reflPainting) (L := R.2) p
-    (l ω).
-
-Definition mkIdReflRestrLayer {n' p ε} {C: νType n'.+1} {G: Dgn C}
-  {Hp: p.+2 <= n'.+2}
-  {FrameBlock: DgnFrameBlock (mkνTypeSn C) p mkDgnFramePrev} {D}
-  {R: mk mkReflPrefix D} {d: mkFramePrev.(Frames) p D} {l: mklayer' d}:
-  rew [mklayer'] FrameBlock.(idReflRestrFrame) (ε := ε) in
-    mkRestrLayer p n' (mkReflLayer l) = l.
-Proof.
-  apply functional_extensionality_dep; intros 𝛉.
-  unfold mkRestrLayer, mkReflLayer.
-  rewrite <-
-    (G.(DgnPainting).(idReflRestrPainting) (L := R.2)
-      (ε := ε) (E := D.2) (c := l 𝛉)).
-  rewrite <- map_subst_app, <- map_subst.
-  rewrite rew_map with
-    (P := fun x => C.(PaintingPrev).(painting') x),
-  rew_map with
-    (P := fun x => C.(PaintingPrev).(painting') x)
-    (f := fun d => C.(Frame).(restrFrame) n' ε d).
-  repeat rewrite rew_compose.
-  apply rew_swap with
-    (P := fun x => C.(PaintingPrev).(painting') x).
-  rewrite rew_app_rl. now trivial.
-  now apply (C.(FramePrev).(Frames) p D.1).(UIP).
-Defined.
-
-Definition mkCohReflRestrLayer {n' p} q {ε} {C: νType n'.+1} {G: Dgn C}
-  {Hp: p.+3 <= q.+3} {Hq: q.+3 <= n'.+2}
-  {FrameBlock: DgnFrameBlock (mkνTypeSn C) p mkDgnFramePrev} {D}
-  {R: mk mkReflPrefix D} {d: mkFramePrev.(Frames) p D} {l: mklayer' (C := C) d}:
-    rew [mklayer'] FrameBlock.(cohReflRestrFrame) q.+1 in
-     G.(ReflLayer) (C.(RestrLayer) p q ε l) = mkRestrLayer p q (mkReflLayer l).
-Proof.
-  apply functional_extensionality_dep; intros 𝛉.
-  unfold RestrLayer, mkRestrLayer, ReflLayer, mkReflLayer.
-  rewrite <- map_subst_app, <- !map_subst.
-  rewrite rew_map with
-    (P := fun x => C.(PaintingPrev).(painting') x),
-  rew_map with
-    (P := fun x => C.(PaintingPrev).(painting') x)
-    (f := fun d => C.(Frame).(restrFrame) q ε d),
-  rew_map with
-    (P := fun x => C.(PaintingPrev).(painting') x)
-    (f := fun x => G.(DgnFramePrev).(reflFrame') p x).
-  rewrite <- (G.(DgnPainting).(cohReflRestrPainting) q (L := R.2)
-    (E := D.2)).
-  repeat rewrite rew_compose.
-  apply rew_swap with
-    (P := fun x => C.(PaintingPrev).(painting') x).
-  rewrite rew_app_rl. now trivial.
-  now apply (C.(FramePrev).(Frames) p D.1).(UIP).
-Defined.
-
-#[local]
-Instance mkDgnFrame0 {n'} {C: νType n'.+1} {G: Dgn C}:
-  DgnFrameBlock (mkνTypeSn C) O mkDgnFramePrev.
-  unshelve esplit.
-  * intros; now exact tt.
-  * intros; apply rew_swap with (P := id); now destruct (rew <- _ in _).
-  * intros; apply rew_swap with (P := id); now destruct (rew _ in _).
-Defined.
-
-#[local]
-Instance mkDgnFrameSp {n' p} {C: νType n'.+1} {G: Dgn C}
-  {Frame: DgnFrameBlock (mkνTypeSn C) p mkDgnFramePrev}:
-  DgnFrameBlock (mkνTypeSn C) p.+1 mkDgnFramePrev.
-  unshelve esplit.
-  * (* reflFrame *)
-    intros Hp D R d'.
-    destruct (rew [id] (mkνTypeSn C).(eqFrameSp') in d') as (d, l); clear d'.
-    now exact (Frame.(reflFrame) d; mkReflLayer l).
-  * (* idReflRestrFrame *)
-    simpl; intros ε Hp D R d'.
-    rewrite <- rew_opp_l with (P := id) (H := C.(eqFrameSp)).
-    destruct (rew [id] _ in d') as (d, l); clear d'.
-    f_equal.
-    now exact (= Frame.(idReflRestrFrame); mkIdReflRestrLayer).
-  * (* cohReflRestrFrame *)
-    intros q ε Hpq Hq D R d'; simpl. invert_le Hpq. invert_le Hq.
-    rewrite <- rew_opp_l with (P := id) (H := C.(eqFrameSp)) (a := d'),
-            rew_opp_r.
-    destruct (rew [id] _ in d') as (d, l); clear d'.
-    rewrite C.(eqRestrFrameSp), G.(eqReflFrameSp).
-    f_equal.
-    now exact (= Frame.(cohReflRestrFrame) q.+1; mkCohReflRestrLayer q).
-Defined.
-
-#[local]
-Instance mkDgnFrame {n' p} {C: νType n'.+1} {G: Dgn C}:
-  DgnFrameBlock (mkνTypeSn C) p mkDgnFramePrev.
-  induction p.
-  * now exact mkDgnFrame0.
-  * now exact mkDgnFrameSp.
-Defined.
-
-#[local]
-Instance mkDgnPaintingPrev {n'} {C: νType n'.+1} {G: Dgn C}:
-  DgnPaintingBlockPrev (mkνTypeSn C) mkDgnFramePrev := {|
-  reflPainting' p Hp (D: (mkνTypeSn C).(prefix)) (R: mk mkReflPrefix D) d c :=
-    G.(DgnPainting).(reflPainting) p c (L := R.2);
-|}.
-
-Definition mkReflPainting {n'} p {C: νType n'.+1} {G: Dgn C}
-  {Hp: p.+1 <= n'.+2} {D} {R: mk mkReflPrefix D} {E} {L: HasRefl E}
-  {d: mkFramePrev.(Frames) p D} (c: mkPaintingPrev.(painting') d):
-  mkPaintingType n'.+1 p E (mkDgnFrame.(reflFrame) d).
-Proof.
-  revert d c; apply le_induction' with (Hp := Hp); clear p Hp.
-  * intros d c. rewrite mkPaintingType_step_computes. unshelve esplit.
-    - now exact (fun ε : arity => rew <- [mkPaintingPrev.(painting')]
-        (mkDgnFrame).(idReflRestrFrame) (ε := ε) in c).
-    - rewrite mkPaintingType_base_computes.
-      now exact (L d c).
-  * intros p Hp IHP d c.
-    destruct (rew [id] C.(eqPaintingSp) in c) as (l, c').
-    simpl in IHP; specialize (IHP (rew <- [id] C.(eqFrameSp) in (d; l)) c').
-    rewrite rew_rew' in IHP.
-    rewrite mkPaintingType_step_computes.
-    unshelve esplit.
-    - now exact (mkReflLayer l).
-    - now apply IHP.
-Defined.
-
-Lemma mkReflPainting_base_computes {n'} {C: νType n'.+1} {G: Dgn C} {D}
-  {R: mk mkReflPrefix D} {E} {L: HasRefl E} {d: mkFramePrev.(Frames) n'.+1 D}
-  {c: mkPaintingPrev.(painting') d}:
-  mkReflPainting n'.+1 (E := E) c =
-  rew <- [id] mkPaintingType_step_computes in
-    ((fun ε : arity => rew <- [mkPaintingPrev.(painting')]
-      (mkDgnFrame).(idReflRestrFrame) (ε := ε) in c);
-    rew <- mkPaintingType_base_computes in L d c).
-Proof.
-  unfold mkReflPainting; now rewrite le_induction'_base_computes.
-Qed.
-
-Lemma mkReflPainting_step_computes {n' p} {C: νType n'.+1} {G: Dgn C}
-  {Hp: p.+2 <= n'.+2} {D} {R: mk mkReflPrefix D}
-  {E} {L: HasRefl E} {d: mkFramePrev.(Frames) p D}
-  {c: mkPaintingPrev.(painting') d}:
-  mkReflPainting p (E := E) c = match (rew [id] C.(eqPaintingSp) in c) with
-  | (l; c') => rew <- [id] mkPaintingType_step_computes in
-    (mkReflLayer l;
-    rew [fun d => mkPaintingType n'.+1 p.+1 E match d with
-          (d'; l) => (mkDgnFrame.(reflFrame) d'; mkReflLayer l)
-        end] rew_rew' C.(eqFrameSp) id in mkReflPainting p.+1 (E := E) c')
-  end.
-Proof.
-  unfold mkReflPainting; now rewrite le_induction'_step_computes.
-Qed.
-
-#[local]
-Instance mkDgnPainting {n'} {C: νType n'.+1} {G: Dgn C}:
-  DgnPaintingBlock (mkνTypeSn C) mkDgnPaintingPrev (fun p => mkDgnFrame).
-  unshelve esplit.
-  - (* reflPainting *)
-    intros. apply mkReflPainting.
-    * now exact L.
-    * now exact X.
-  - (* idReflRestrPainting *)
-    intros. revert d c. pattern p, Hp; apply le_induction'; clear p Hp.
-    * intros d c; simpl (mkνTypeSn C).(Painting).(restrPainting); cbv beta.
-      rewrite mkRestrPainting_base_computes, mkReflPainting_base_computes.
-      now repeat rewrite rew_rew'.
-    * intros p Hp IHP d c. simpl.
-      rewrite mkRestrPainting_step_computes, mkReflPainting_step_computes.
-      (* Coq bug? Why doesn't a direct destruct work? *)
-      transitivity (rew <- [id] C.(eqPaintingSp) in rew [id] C.(eqPaintingSp) in c).
-      2: now rewrite rew_rew.
-      set (c' := rew [id] C.(eqPaintingSp) in c).
-      change (rew [id] C.(eqPaintingSp) in c) with c'.
-      destruct c' as (l, c''). clear c; rename c'' into c.
-      rewrite rew_rew'.
-      rewrite <- rew_permute_rl with (H := C.(@eqPaintingSp _) _ _ _ _).
-      f_equal.
-      unshelve eapply (rew_existT_curried
-        (Q := fun x =>
-          C.(Painting).(painting) _ (rew <- [id] C.(eqFrameSp) in x))).
-      + now exact mkIdReflRestrLayer.
-      + rewrite <- IHP,
-                rew_map with
-                  (P := fun x => C.(Painting).(painting) D.2 x)
-                  (f := fun x => rew <- [id] C.(eqFrameSp) in x).
-        apply rew_swap_rl with (P := C.(Painting).(painting) D.2).
-        rewrite rew_compose.
-        simpl (mkνTypeSn C).(Painting).(restrPainting). cbv beta.
-        set (h := fun d => match d with (d'; l') =>
-            (mkDgnFrame.(reflFrame) d' as a in (mkFrame p).(frame _) D;
-             mkReflLayer l' in mkLayer a)
-            end).
-        set (e' := rew_rew' _ _);
-        rewrite <- (map_subst (P := fun d => mkPaintingType n'.+1 p.+1 E (h d))
-            (fun d c => mkRestrPainting p.+1 n'.+1 E _ c) e' _); subst e'.
-        rewrite rew_map with
-            (P := fun x => (mkPaintingPrev.(painting') x).(Dom))
-            (f := fun x => (mkFrame p.+1).(restrFrame) n'.+1 _ (h x)).
-        apply rew_swap_rl with (P := C.(Painting).(painting) D.2),
-              rew_app_rl_opp with (P := fun x => C.(Painting).(painting) D.2 x).
-        now apply (C.(Frame).(frame p.+1) D.1).(UIP).
-  - (* cohReflRestrPainting *)
-    intros; simpl.
-    revert d c. pattern p, Hpq; apply le_induction''; clear p Hpq.
-    * intros d c; simpl.
-      rewrite mkRestrPainting_base_computes, mkReflPainting_step_computes.
-      set (c' := rew [id] C.(eqPaintingSp) in c).
-      change (rew [id] C.(eqPaintingSp) in c) with c'.
-      replace c with (rew <- [id] C.(eqPaintingSp) in c') by apply rew_rew.
-      destruct c' as (l, c''); clear c; rename c'' into c.
-      rewrite rew_rew', rew_rew.
-      now rewrite (C.(eqRestrPainting0) c).
-    * intros p Hp IHP d c; simpl. invert_le Hp.
-      rewrite mkRestrPainting_step_computes, mkReflPainting_step_computes.
-      set (c' := rew [id] C.(eqPaintingSp) in c).
-      change (rew [id] C.(eqPaintingSp) in c) with c'.
-      replace c with (rew <- [id] C.(eqPaintingSp) in c') by apply rew_rew.
-      destruct c' as (l, c''); clear c; rename c'' into c.
-      rewrite rew_rew',
-              (C.(eqRestrPaintingSp) p q),
-              (G.(eqReflPaintingSp) p q),
-              <- rew_permute_rr with (H := C.(@eqPaintingSp _) _ _ _ _).
-      f_equal.
-      unshelve eapply (rew_existT_curried
-        (Q := fun x =>
-          C.(Painting).(painting) _ (rew <- [id] C.(eqFrameSp) in x))).
-      + now rewrite <- mkCohReflRestrLayer with (d := d), rew_compose,
-                       eq_trans_sym_inv_r.
-      + rewrite <- map_subst, <- IHP.
-        apply rew_swap_rl with
-            (P := fun x => C.(Painting).(painting) D.2
-            (rew <- [id] C.(eqFrameSp) in x)).
-        set (h := fun d => match d with (d'; l') =>
-            (mkDgnFrame.(reflFrame) d' as a in (mkFrame p).(frame _) D;
-             mkReflLayer l' in mkLayer a)
-            end).
-        set (e' := rew_rew' _ _);
-        rewrite <- (map_subst (P := fun d => mkPaintingType n'.+1 p.+1 E (h d))
-            (fun d c => mkRestrPainting p.+1 q.+1 E _ c) e' _); subst e'.
-        set (P := fun x => (C.(Painting).(painting) D.2 x).(Dom)).
-        rewrite rew_map with (P := P) (f := G.(DgnFrame).(reflFrame)),
-                rew_map' with (P := P)
-                  (f := fun x => rew <- [id] C.(eqFrameSp) in x),
-                rew_map with (P := P)
-                  (f := fun d => ((mkFrame p.+1).(restrFrame) q.+1 ε (h d))).
-        apply rew_swap_rl with (P := P).
-        rewrite rew_compose_rl,
-                rew_compose_lr with (P := P).
-        set (t0 := eq_trans _ _); set (t1 := eq_trans _ _);
-        clearbody t0; clearbody t1.
-        repeat rewrite rew_compose.
-        now rewrite ((C.(Frame).(frame p.+1) D.1).(UIP)
-            (h := eq_trans _ _) (g := eq_refl)).
-Defined.
-
-#[local]
-Instance mkDgn0: Dgn (νTypeAt 1).
-Proof.
-  unshelve esplit.
-  - intro. now exact hunit.
-  - split; intros; now le_contra Hp.
-  - intros; unshelve esplit.
-    * simpl; intros; invert_le Hp. now exact tt.
-    * simpl; intros; invert_le Hp; destruct d. now exact eq_refl.
-    * simpl; intros; now le_contra Hq.
-  - split; intros; now le_contra Hp.
-  - intros; unshelve esplit.
-    * simpl; intros * L * c; invert_le Hp; destruct d.
-      rewrite mkPaintingType_step_computes. unshelve esplit. now trivial.
-      rewrite mkPaintingType_base_computes. now exact (L tt c).
-    * simpl; intros; invert_le Hp; destruct d. simpl.
-      now rewrite mkRestrPainting_base_computes, rew_rew'.
-    * simpl; intros; now le_contra Hq.
-  - intros; now le_contra Hq.
-  - intros; now le_contra Hq.
-Defined.
-
-#[local]
-Instance mkDgnSn {n'} {C: νType n'.+1}:
-  Dgn C -> Dgn (mkνTypeSn C).
-Proof.
-  unshelve esplit.
-  - intros; simpl; now rewrite rew_rew'.
-  - intros; simpl. rewrite mkReflPainting_step_computes, rew_rew'.
-    change (eq_ind_r (x := ?x) ?P) with (eq_rect_r (x := x) P).
-    now rewrite rew_map with (P := mkPaintingType n'.+1 p.+1 E), rew_eq_refl.
-Defined.
-
-Fixpoint νDgnTypeAt n': Dgn (νTypeAt n'.+1) :=
-  match n' with
-  | O => mkDgn0
-  | n'.+1 => mkDgnSn (νDgnTypeAt n')
-  end.
-
-CoInductive νDgnTypeFrom n' (X: (νTypeAt n'.+1).(prefix)) (M: νTypeFrom n'.+1 X)
-  (L: (νDgnTypeAt n').(ReflPrefix) X): Type@{m'} := cons' {
-  dgn: HasRefl M.(this);
-  dgnNext: νDgnTypeFrom n'.+1 (X; M.(this)) M.(next) (L; dgn);
-}.
-
-Definition νDgnTypes (X: νTypes) := νDgnTypeFrom 0 (tt; X.(this)) X.(next) tt.
 End νType.
-
-Definition AugmentedSemiSimplicial := νTypes hunit.
-Definition SemiSimplicial := νTypeFrom hunit 1 (tt; fun _ => hunit).
-Definition SemiCubical := νTypes hbool.
-Definition AugmentedSimplicial := { X &_T νDgnTypes hunit X }.
-Definition Cubical := { X &_T νDgnTypes hbool X }.
-
-(** Some examples *)
-
-Notation "{ x : A && P }" := (sigT (A := A) (fun x => P)): type_scope.
-
-Example SemiSimplicial2 := Eval lazy -[projT2] in
- (νTypeAt hunit 2).(prefix _).
-Print SemiSimplicial2.
-
-Example SemiCubical2 := Eval lazy -[projT2] in
- (νTypeAt hbool 2).(prefix _).
-Print SemiCubical2.
-
-Example Simplicial1 := Eval lazy -[projT1 projT2] in
- (νDgnTypeAt hunit 1).(ReflPrefix _).
-Print Simplicial1.
-
-Example Cubical1 := Eval lazy -[projT1 projT2] in
- (νDgnTypeAt hbool 1).(ReflPrefix _).
-Print Cubical1.
